WIP

ovn/proofs/ssprove/extraction/Hacspec_ovn.v
@@ -27,81 +27,128 @@ Obligation Tactic := (* try timeout 8 *) solve_ssprove_obligations.
 Require Import Hacspec_ovn_Ovn_traits.
 Export Hacspec_ovn_Ovn_traits.
 
-(*Not implemented yet? todo(item)*)
+(*** Remove locations *)
+
+Notation both0 := (both (fset []) (fset [])).
 
 (*Not implemented yet? todo(item)*)
 
 (*Not implemented yet? todo(item)*)
 
-Equations compute_group_element_for_vote {v_Z : _} {v_G : _} `{ t_Sized (v_Z)} `{ t_Sized (v_G)} `{ t_Z_Field (v_Z)} `{ t_Group (v_G) (v_Z)} (xi : both (f_field_type)) (vote : both ('bool)) (g_pow_yi : both (f_group_type)) : both (f_group_type) :=
+(*Not implemented yet? todo(item)*)
+
+Program Definition if_both0 {A} (c : both0 'bool) (e_then : both0 A) (e_else : both0 A) : both0 A :=
+  bind_both (fsubset_loc := _) (fsubset_opsig := _) c (fun b => if b then lift_both (fsubset_loc := _) (fsubset_opsig := _) e_then else lift_both  (fsubset_loc := _) (fsubset_opsig := _) e_else).
+Solve All Obligations with solve_ssprove_obligations.
+Fail Next Obligation.
+
+Notation "'ifb0' b 'then' et 'else' ee" := (if_both0 b et ee).
+(* Notation "f_prod". *)
+
+Equations foldi_both_list0
+           {acc B: choice_type}
+        (l : both0 (chList B))
+        (f: both0 B ->
+            both0 acc ->
+            both0 acc)
+        (init: both0 acc)
+  : both0 (acc) :=
+  foldi_both_list0 l f init :=
+  bind_both l (fun l' => List.fold_left (fun x y => solve_lift @f (solve_lift ret_both y) (x) : both0 _) l' (solve_lift init)).
+Solve All Obligations with intros ; solve_fsubset_trans.
+Solve All Obligations with intros ; solve_ssprove_obligations.
+Fail Next Obligation.
+
+Equations prod_both0 {ceA ceB : choice_type} (a : both0 ceA) (b : both0 ceB) : both0 (ceA × ceB) :=
+  prod_both0 a b :=
+    bind_both a (fun a' =>
+    bind_both b (fun b' =>
+                   (ret_both ((a', b') : _ × _)))).
+Solve All Obligations with intros ; solve_in_fset.
+Fail Next Obligation.
+
+Definition Build_t_Range {WS} {f_start : both0 (int WS)} {f_end : both0 (int WS)} : both0 (chProd (int WS) (int WS)) := @prod_both0 (int WS) (int WS) f_start f_end.
+(* Class iterable (A B : choice_type) := {f_into_iter : both0 A -> both0 (chList B)}. *)
+
+(* Equations array_index *)
+(*   {A: choice_type} {len : nat} (x : both0 (nseq_ A len)) {WS} (y : both0 (int WS)) : both0 A := *)
+(*   array_index x (WS := WS) y := solve_lift lift2_both (fun x y => Hacspec_Lib_Pre.array_index x y) x y. *)
+(* Fail Next Obligation. *)
+
+Notation " x '.a[' a ']'" := (solve_lift array_index (n_seq_array_or_seq x _) a : both0 _) (at level 40).
+
+
+(** End *)
+
+Equations compute_group_element_for_vote {v_Z : _} {v_G : _} `{ t_Sized (v_Z)} `{ t_Sized (v_G)} `{ t_Z_Field (v_Z)} `{ t_Group (v_G) (v_Z)} (xi : both0 (f_field_type)) (vote : both0 ('bool)) (g_pow_yi : both0 (f_group_type)) : both0 (f_group_type) :=
   compute_group_element_for_vote xi vote g_pow_yi  :=
-    solve_lift (f_prod (f_pow g_pow_yi xi) (f_g_pow (ifb vote
-    then f_field_one (ret_both (tt : 'unit))
-    else f_field_zero (ret_both (tt : 'unit))))) : both (f_group_type).
+    solve_lift (f_prod (f_pow g_pow_yi xi) (f_g_pow (ifb0 vote
+    then f_field_one
+    else f_field_zero))) : both0 (f_group_type).
 Fail Next Obligation.
 
-Equations select_private_voting_key {v_Z : _} `{ t_Sized (v_Z)} `{ t_Z_Field (v_Z)} (random : both (int32)) : both (f_field_type) :=
+Equations select_private_voting_key {v_Z : _} `{ t_Sized (v_Z)} `{ t_Z_Field (v_Z)} (random : both0 (int32)) : both0 (f_field_type) :=
   select_private_voting_key random  :=
-    solve_lift (f_random_field_elem random) : both (f_field_type).
+    solve_lift (f_random_field_elem random) : both0 (f_field_type).
 Fail Next Obligation.
-
-Equations compute_g_pow_yi {v_Z : _} {v_G : _} {n : both (uint_size)} `{ t_Sized (v_Z)} `{ t_Sized (v_G)} `{ t_Z_Field (v_Z)} `{ t_Group (v_G) (v_Z)} (i : both (uint_size)) (xis : both (nseq f_group_type (is_pure (n)))) : both (f_group_type) :=
+  
+Equations compute_g_pow_yi {v_Z : _} {v_G : _} {n : both0 (uint_size)} `{ t_Sized (v_Z)} `{ t_Sized (v_G)} `{ t_Z_Field (v_Z)} `{ t_Group (v_G) (v_Z)} (i : both0 (uint_size)) (xis : both0 (nseq f_group_type (is_pure (n)))) : both0 (f_group_type) :=
   compute_g_pow_yi i xis  :=
-    letb prod1 := f_group_one (ret_both (tt : 'unit)) in
-    letb prod1 := foldi_both_list (f_into_iter (Build_t_Range (f_start := ret_both (0 : uint_size)) (f_end := i))) (fun j =>
+    letb prod1 := f_group_one in
+    letb prod1 := foldi_both_list0 (f_into_iter (Build_t_Range (f_start := solve_lift ret_both (0 : uint_size)) (f_end := i))) (fun j =>
       ssp (fun prod1 =>
-        solve_lift (f_prod prod1 (xis.a[j])) : both (f_group_type))) prod1 in
-    letb prod2 := f_group_one (ret_both (tt : 'unit)) in
-    letb prod2 := foldi_both_list (f_into_iter (Build_t_Range (f_start := i .+ (ret_both (1 : uint_size))) (f_end := n))) (fun j =>
+        (* solve_lift (f_prod prod1 (xis.a[j])) : both0 (f_group_type) *) _)) prod1 in
+    letb prod2 := f_group_one in
+    letb prod2 := foldi_both0_list (f_into_iter (Build_t_Range (f_start := (* i .+ (ret_both (1 : uint_size)) *)_ ) (f_end := n))) (fun j =>
       ssp (fun prod2 =>
-        solve_lift (f_prod prod2 (xis.a[j])) : both (f_group_type))) prod2 in
-    solve_lift (f_div prod1 prod2) : both (f_group_type).
+        solve_lift (f_prod prod2 (xis.a[j])) : both0 (f_group_type))) prod2 in
+    solve_lift (f_div prod1 prod2) : both0 (f_group_type).
 Solve All Obligations with now intros ; destruct from_uint_size.
 Fail Next Obligation.
 
-Equations check_commitment {v_Z : _} {v_G : _} `{ t_Sized (v_Z)} `{ t_Sized (v_G)} `{ t_Z_Field (v_Z)} `{ t_Group (v_G) (v_Z)} (g_pow_xi_yi_vi : both (f_group_type)) (commitment : both (f_field_type)) : both ('bool) :=
+Equations check_commitment {v_Z : _} {v_G : _} `{ t_Sized (v_Z)} `{ t_Sized (v_G)} `{ t_Z_Field (v_Z)} `{ t_Group (v_G) (v_Z)} (g_pow_xi_yi_vi : both0 (f_group_type)) (commitment : both0 (f_field_type)) : both0 ('bool) :=
   check_commitment g_pow_xi_yi_vi commitment  :=
-    solve_lift ((f_hash (impl__into_vec (unsize (box_new (array_from_list [g_pow_xi_yi_vi]))))) =.? commitment) : both ('bool).
+    solve_lift ((f_hash (impl__into_vec (unsize (box_new (array_from_list [g_pow_xi_yi_vi]))))) =.? commitment) : both0 ('bool).
 Fail Next Obligation.
 
-Equations commit_to {v_Z : _} {v_G : _} `{ t_Sized (v_Z)} `{ t_Sized (v_G)} `{ t_Z_Field (v_Z)} `{ t_Group (v_G) (v_Z)} (g_pow_xi_yi_vi : both (f_group_type)) : both (f_field_type) :=
+Equations commit_to {v_Z : _} {v_G : _} `{ t_Sized (v_Z)} `{ t_Sized (v_G)} `{ t_Z_Field (v_Z)} `{ t_Group (v_G) (v_Z)} (g_pow_xi_yi_vi : both0 (f_group_type)) : both0 (f_field_type) :=
   commit_to g_pow_xi_yi_vi  :=
-    solve_lift (f_hash (impl__into_vec (unsize (box_new (array_from_list [g_pow_xi_yi_vi]))))) : both (f_field_type).
+    solve_lift (f_hash (impl__into_vec (unsize (box_new (array_from_list [g_pow_xi_yi_vi]))))) : both0 (f_field_type).
 Fail Next Obligation.
 
 Definition t_CastVoteParam {v_Z : _} `{ t_Sized (v_Z)} `{ t_Z_Field (v_Z)} : choice_type :=
   (int32 × f_field_type × int32 × int32 × int32 × 'bool).
-Equations f_cvp_i {v_Z : _} `{ t_Sized (v_Z)} `{ t_Z_Field (v_Z)} (s : both (t_CastVoteParam)) : both (int32) :=
+Equations f_cvp_i {v_Z : _} `{ t_Sized (v_Z)} `{ t_Z_Field (v_Z)} (s : both0 (t_CastVoteParam)) : both0 (int32) :=
   f_cvp_i s  :=
     bind_both s (fun x =>
-      solve_lift (ret_both (fst (fst (fst (fst (fst x)))) : int32))) : both (int32).
+      solve_lift (ret_both (fst (fst (fst (fst (fst x)))) : int32))) : both0 (int32).
 Fail Next Obligation.
-Equations f_cvp_xi {v_Z : _} `{ t_Sized (v_Z)} `{ t_Z_Field (v_Z)} (s : both (t_CastVoteParam)) : both (f_field_type) :=
+Equations f_cvp_xi {v_Z : _} `{ t_Sized (v_Z)} `{ t_Z_Field (v_Z)} (s : both0 (t_CastVoteParam)) : both0 (f_field_type) :=
   f_cvp_xi s  :=
     bind_both s (fun x =>
-      solve_lift (ret_both (snd (fst (fst (fst (fst x)))) : f_field_type))) : both (f_field_type).
+      solve_lift (ret_both (snd (fst (fst (fst (fst x)))) : f_field_type))) : both0 (f_field_type).
 Fail Next Obligation.
-Equations f_cvp_zkp_random_w {v_Z : _} `{ t_Sized (v_Z)} `{ t_Z_Field (v_Z)} (s : both (t_CastVoteParam)) : both (int32) :=
+Equations f_cvp_zkp_random_w {v_Z : _} `{ t_Sized (v_Z)} `{ t_Z_Field (v_Z)} (s : both0 (t_CastVoteParam)) : both0 (int32) :=
   f_cvp_zkp_random_w s  :=
     bind_both s (fun x =>
-      solve_lift (ret_both (snd (fst (fst (fst x))) : int32))) : both (int32).
+      solve_lift (ret_both (snd (fst (fst (fst x))) : int32))) : both0 (int32).
 Fail Next Obligation.
-Equations f_cvp_zkp_random_r {v_Z : _} `{ t_Sized (v_Z)} `{ t_Z_Field (v_Z)} (s : both (t_CastVoteParam)) : both (int32) :=
+Equations f_cvp_zkp_random_r {v_Z : _} `{ t_Sized (v_Z)} `{ t_Z_Field (v_Z)} (s : both0 (t_CastVoteParam)) : both0 (int32) :=
   f_cvp_zkp_random_r s  :=
     bind_both s (fun x =>
-      solve_lift (ret_both (snd (fst (fst x)) : int32))) : both (int32).
+      solve_lift (ret_both (snd (fst (fst x)) : int32))) : both0 (int32).
 Fail Next Obligation.
-Equations f_cvp_zkp_random_d {v_Z : _} `{ t_Sized (v_Z)} `{ t_Z_Field (v_Z)} (s : both (t_CastVoteParam)) : both (int32) :=
+Equations f_cvp_zkp_random_d {v_Z : _} `{ t_Sized (v_Z)} `{ t_Z_Field (v_Z)} (s : both0 (t_CastVoteParam)) : both0 (int32) :=
   f_cvp_zkp_random_d s  :=
     bind_both s (fun x =>
-      solve_lift (ret_both (snd (fst x) : int32))) : both (int32).
+      solve_lift (ret_both (snd (fst x) : int32))) : both0 (int32).
 Fail Next Obligation.
-Equations f_cvp_vote {v_Z : _} `{ t_Sized (v_Z)} `{ t_Z_Field (v_Z)} (s : both (t_CastVoteParam)) : both ('bool) :=
+Equations f_cvp_vote {v_Z : _} `{ t_Sized (v_Z)} `{ t_Z_Field (v_Z)} (s : both0 (t_CastVoteParam)) : both0 ('bool) :=
   f_cvp_vote s  :=
     bind_both s (fun x =>
-      solve_lift (ret_both (snd x : 'bool))) : both ('bool).
+      solve_lift (ret_both (snd x : 'bool))) : both0 ('bool).
 Fail Next Obligation.
-Equations Build_t_CastVoteParam {v_Z : _} `{ t_Sized (v_Z)} `{ t_Z_Field (v_Z)} {f_cvp_i : both (int32)} {f_cvp_xi : both (f_field_type)} {f_cvp_zkp_random_w : both (int32)} {f_cvp_zkp_random_r : both (int32)} {f_cvp_zkp_random_d : both (int32)} {f_cvp_vote : both ('bool)} : both (t_CastVoteParam) :=
+Equations Build_t_CastVoteParam {v_Z : _} `{ t_Sized (v_Z)} `{ t_Z_Field (v_Z)} {f_cvp_i : both0 (int32)} {f_cvp_xi : both0 (f_field_type)} {f_cvp_zkp_random_w : both0 (int32)} {f_cvp_zkp_random_r : both0 (int32)} {f_cvp_zkp_random_d : both0 (int32)} {f_cvp_vote : both0 ('bool)} : both0 (t_CastVoteParam) :=
   Build_t_CastVoteParam  :=
     bind_both f_cvp_vote (fun f_cvp_vote =>
       bind_both f_cvp_zkp_random_d (fun f_cvp_zkp_random_d =>
@@ -109,7 +156,7 @@ Equations Build_t_CastVoteParam {v_Z : _} `{ t_Sized (v_Z)} `{ t_Z_Field (v_Z)} 
           bind_both f_cvp_zkp_random_w (fun f_cvp_zkp_random_w =>
             bind_both f_cvp_xi (fun f_cvp_xi =>
               bind_both f_cvp_i (fun f_cvp_i =>
-                solve_lift (ret_both ((f_cvp_i,f_cvp_xi,f_cvp_zkp_random_w,f_cvp_zkp_random_r,f_cvp_zkp_random_d,f_cvp_vote) : (t_CastVoteParam))))))))) : both (t_CastVoteParam).
+                solve_lift (ret_both ((f_cvp_i,f_cvp_xi,f_cvp_zkp_random_w,f_cvp_zkp_random_r,f_cvp_zkp_random_d,f_cvp_vote) : (t_CastVoteParam))))))))) : both0 (t_CastVoteParam).
 Fail Next Obligation.
 Notation "'Build_t_CastVoteParam' '[' x ']' '(' 'f_cvp_i' ':=' y ')'" := (Build_t_CastVoteParam (f_cvp_i := y) (f_cvp_xi := f_cvp_xi x) (f_cvp_zkp_random_w := f_cvp_zkp_random_w x) (f_cvp_zkp_random_r := f_cvp_zkp_random_r x) (f_cvp_zkp_random_d := f_cvp_zkp_random_d x) (f_cvp_vote := f_cvp_vote x)).
 Notation "'Build_t_CastVoteParam' '[' x ']' '(' 'f_cvp_xi' ':=' y ')'" := (Build_t_CastVoteParam (f_cvp_i := f_cvp_i x) (f_cvp_xi := y) (f_cvp_zkp_random_w := f_cvp_zkp_random_w x) (f_cvp_zkp_random_r := f_cvp_zkp_random_r x) (f_cvp_zkp_random_d := f_cvp_zkp_random_d x) (f_cvp_vote := f_cvp_vote x)).
@@ -120,62 +167,62 @@ Notation "'Build_t_CastVoteParam' '[' x ']' '(' 'f_cvp_vote' ':=' y ')'" := (Bui
 
 Definition t_OrZKPCommit {v_Z : _} {v_G : _} `{ t_Sized (v_Z)} `{ t_Sized (v_G)} `{ t_Z_Field (v_Z)} `{ t_Group (v_G) (v_Z)} : choice_type :=
   (f_group_type × f_group_type × f_group_type × f_group_type × f_group_type × f_group_type × f_field_type × f_field_type × f_field_type × f_field_type × f_field_type).
-Equations f_or_zkp_x {v_Z : _} {v_G : _} `{ t_Sized (v_Z)} `{ t_Sized (v_G)} `{ t_Z_Field (v_Z)} `{ t_Group (v_G) (v_Z)} (s : both (t_OrZKPCommit)) : both (f_group_type) :=
+Equations f_or_zkp_x {v_Z : _} {v_G : _} `{ t_Sized (v_Z)} `{ t_Sized (v_G)} `{ t_Z_Field (v_Z)} `{ t_Group (v_G) (v_Z)} (s : both0 (t_OrZKPCommit)) : both0 (f_group_type) :=
   f_or_zkp_x s  :=
     bind_both s (fun x =>
-      solve_lift (ret_both (fst (fst (fst (fst (fst (fst (fst (fst (fst (fst x))))))))) : f_group_type))) : both (f_group_type).
+      solve_lift (ret_both (fst (fst (fst (fst (fst (fst (fst (fst (fst (fst x))))))))) : f_group_type))) : both0 (f_group_type).
 Fail Next Obligation.
-Equations f_or_zkp_y {v_Z : _} {v_G : _} `{ t_Sized (v_Z)} `{ t_Sized (v_G)} `{ t_Z_Field (v_Z)} `{ t_Group (v_G) (v_Z)} (s : both (t_OrZKPCommit)) : both (f_group_type) :=
+Equations f_or_zkp_y {v_Z : _} {v_G : _} `{ t_Sized (v_Z)} `{ t_Sized (v_G)} `{ t_Z_Field (v_Z)} `{ t_Group (v_G) (v_Z)} (s : both0 (t_OrZKPCommit)) : both0 (f_group_type) :=
   f_or_zkp_y s  :=
     bind_both s (fun x =>
-      solve_lift (ret_both (snd (fst (fst (fst (fst (fst (fst (fst (fst (fst x))))))))) : f_group_type))) : both (f_group_type).
+      solve_lift (ret_both (snd (fst (fst (fst (fst (fst (fst (fst (fst (fst x))))))))) : f_group_type))) : both0 (f_group_type).
 Fail Next Obligation.
-Equations f_or_zkp_a1 {v_Z : _} {v_G : _} `{ t_Sized (v_Z)} `{ t_Sized (v_G)} `{ t_Z_Field (v_Z)} `{ t_Group (v_G) (v_Z)} (s : both (t_OrZKPCommit)) : both (f_group_type) :=
+Equations f_or_zkp_a1 {v_Z : _} {v_G : _} `{ t_Sized (v_Z)} `{ t_Sized (v_G)} `{ t_Z_Field (v_Z)} `{ t_Group (v_G) (v_Z)} (s : both0 (t_OrZKPCommit)) : both0 (f_group_type) :=
   f_or_zkp_a1 s  :=
     bind_both s (fun x =>
-      solve_lift (ret_both (snd (fst (fst (fst (fst (fst (fst (fst (fst x)))))))) : f_group_type))) : both (f_group_type).
+      solve_lift (ret_both (snd (fst (fst (fst (fst (fst (fst (fst (fst x)))))))) : f_group_type))) : both0 (f_group_type).
 Fail Next Obligation.
-Equations f_or_zkp_b1 {v_Z : _} {v_G : _} `{ t_Sized (v_Z)} `{ t_Sized (v_G)} `{ t_Z_Field (v_Z)} `{ t_Group (v_G) (v_Z)} (s : both (t_OrZKPCommit)) : both (f_group_type) :=
+Equations f_or_zkp_b1 {v_Z : _} {v_G : _} `{ t_Sized (v_Z)} `{ t_Sized (v_G)} `{ t_Z_Field (v_Z)} `{ t_Group (v_G) (v_Z)} (s : both0 (t_OrZKPCommit)) : both0 (f_group_type) :=
   f_or_zkp_b1 s  :=
     bind_both s (fun x =>
-      solve_lift (ret_both (snd (fst (fst (fst (fst (fst (fst (fst x))))))) : f_group_type))) : both (f_group_type).
+      solve_lift (ret_both (snd (fst (fst (fst (fst (fst (fst (fst x))))))) : f_group_type))) : both0 (f_group_type).
 Fail Next Obligation.
-Equations f_or_zkp_a2 {v_Z : _} {v_G : _} `{ t_Sized (v_Z)} `{ t_Sized (v_G)} `{ t_Z_Field (v_Z)} `{ t_Group (v_G) (v_Z)} (s : both (t_OrZKPCommit)) : both (f_group_type) :=
+Equations f_or_zkp_a2 {v_Z : _} {v_G : _} `{ t_Sized (v_Z)} `{ t_Sized (v_G)} `{ t_Z_Field (v_Z)} `{ t_Group (v_G) (v_Z)} (s : both0 (t_OrZKPCommit)) : both0 (f_group_type) :=
   f_or_zkp_a2 s  :=
     bind_both s (fun x =>
-      solve_lift (ret_both (snd (fst (fst (fst (fst (fst (fst x)))))) : f_group_type))) : both (f_group_type).
+      solve_lift (ret_both (snd (fst (fst (fst (fst (fst (fst x)))))) : f_group_type))) : both0 (f_group_type).
 Fail Next Obligation.
-Equations f_or_zkp_b2 {v_Z : _} {v_G : _} `{ t_Sized (v_Z)} `{ t_Sized (v_G)} `{ t_Z_Field (v_Z)} `{ t_Group (v_G) (v_Z)} (s : both (t_OrZKPCommit)) : both (f_group_type) :=
+Equations f_or_zkp_b2 {v_Z : _} {v_G : _} `{ t_Sized (v_Z)} `{ t_Sized (v_G)} `{ t_Z_Field (v_Z)} `{ t_Group (v_G) (v_Z)} (s : both0 (t_OrZKPCommit)) : both0 (f_group_type) :=
   f_or_zkp_b2 s  :=
     bind_both s (fun x =>
-      solve_lift (ret_both (snd (fst (fst (fst (fst (fst x))))) : f_group_type))) : both (f_group_type).
+      solve_lift (ret_both (snd (fst (fst (fst (fst (fst x))))) : f_group_type))) : both0 (f_group_type).
 Fail Next Obligation.
-Equations f_or_zkp_c {v_Z : _} {v_G : _} `{ t_Sized (v_Z)} `{ t_Sized (v_G)} `{ t_Z_Field (v_Z)} `{ t_Group (v_G) (v_Z)} (s : both (t_OrZKPCommit)) : both (f_field_type) :=
+Equations f_or_zkp_c {v_Z : _} {v_G : _} `{ t_Sized (v_Z)} `{ t_Sized (v_G)} `{ t_Z_Field (v_Z)} `{ t_Group (v_G) (v_Z)} (s : both0 (t_OrZKPCommit)) : both0 (f_field_type) :=
   f_or_zkp_c s  :=
     bind_both s (fun x =>
-      solve_lift (ret_both (snd (fst (fst (fst (fst x)))) : f_field_type))) : both (f_field_type).
+      solve_lift (ret_both (snd (fst (fst (fst (fst x)))) : f_field_type))) : both0 (f_field_type).
 Fail Next Obligation.
-Equations f_or_zkp_d1 {v_Z : _} {v_G : _} `{ t_Sized (v_Z)} `{ t_Sized (v_G)} `{ t_Z_Field (v_Z)} `{ t_Group (v_G) (v_Z)} (s : both (t_OrZKPCommit)) : both (f_field_type) :=
+Equations f_or_zkp_d1 {v_Z : _} {v_G : _} `{ t_Sized (v_Z)} `{ t_Sized (v_G)} `{ t_Z_Field (v_Z)} `{ t_Group (v_G) (v_Z)} (s : both0 (t_OrZKPCommit)) : both0 (f_field_type) :=
   f_or_zkp_d1 s  :=
     bind_both s (fun x =>
-      solve_lift (ret_both (snd (fst (fst (fst x))) : f_field_type))) : both (f_field_type).
+      solve_lift (ret_both (snd (fst (fst (fst x))) : f_field_type))) : both0 (f_field_type).
 Fail Next Obligation.
-Equations f_or_zkp_d2 {v_Z : _} {v_G : _} `{ t_Sized (v_Z)} `{ t_Sized (v_G)} `{ t_Z_Field (v_Z)} `{ t_Group (v_G) (v_Z)} (s : both (t_OrZKPCommit)) : both (f_field_type) :=
+Equations f_or_zkp_d2 {v_Z : _} {v_G : _} `{ t_Sized (v_Z)} `{ t_Sized (v_G)} `{ t_Z_Field (v_Z)} `{ t_Group (v_G) (v_Z)} (s : both0 (t_OrZKPCommit)) : both0 (f_field_type) :=
   f_or_zkp_d2 s  :=
     bind_both s (fun x =>
-      solve_lift (ret_both (snd (fst (fst x)) : f_field_type))) : both (f_field_type).
+      solve_lift (ret_both (snd (fst (fst x)) : f_field_type))) : both0 (f_field_type).
 Fail Next Obligation.
-Equations f_or_zkp_r1 {v_Z : _} {v_G : _} `{ t_Sized (v_Z)} `{ t_Sized (v_G)} `{ t_Z_Field (v_Z)} `{ t_Group (v_G) (v_Z)} (s : both (t_OrZKPCommit)) : both (f_field_type) :=
+Equations f_or_zkp_r1 {v_Z : _} {v_G : _} `{ t_Sized (v_Z)} `{ t_Sized (v_G)} `{ t_Z_Field (v_Z)} `{ t_Group (v_G) (v_Z)} (s : both0 (t_OrZKPCommit)) : both0 (f_field_type) :=
   f_or_zkp_r1 s  :=
     bind_both s (fun x =>
-      solve_lift (ret_both (snd (fst x) : f_field_type))) : both (f_field_type).
+      solve_lift (ret_both (snd (fst x) : f_field_type))) : both0 (f_field_type).
 Fail Next Obligation.
-Equations f_or_zkp_r2 {v_Z : _} {v_G : _} `{ t_Sized (v_Z)} `{ t_Sized (v_G)} `{ t_Z_Field (v_Z)} `{ t_Group (v_G) (v_Z)} (s : both (t_OrZKPCommit)) : both (f_field_type) :=
+Equations f_or_zkp_r2 {v_Z : _} {v_G : _} `{ t_Sized (v_Z)} `{ t_Sized (v_G)} `{ t_Z_Field (v_Z)} `{ t_Group (v_G) (v_Z)} (s : both0 (t_OrZKPCommit)) : both0 (f_field_type) :=
   f_or_zkp_r2 s  :=
     bind_both s (fun x =>
-      solve_lift (ret_both (snd x : f_field_type))) : both (f_field_type).
+      solve_lift (ret_both (snd x : f_field_type))) : both0 (f_field_type).
 Fail Next Obligation.
-Equations Build_t_OrZKPCommit {v_Z : _} {v_G : _} `{ t_Sized (v_Z)} `{ t_Sized (v_G)} `{ t_Z_Field (v_Z)} `{ t_Group (v_G) (v_Z)} {f_or_zkp_x : both (f_group_type)} {f_or_zkp_y : both (f_group_type)} {f_or_zkp_a1 : both (f_group_type)} {f_or_zkp_b1 : both (f_group_type)} {f_or_zkp_a2 : both (f_group_type)} {f_or_zkp_b2 : both (f_group_type)} {f_or_zkp_c : both (f_field_type)} {f_or_zkp_d1 : both (f_field_type)} {f_or_zkp_d2 : both (f_field_type)} {f_or_zkp_r1 : both (f_field_type)} {f_or_zkp_r2 : both (f_field_type)} : both (t_OrZKPCommit) :=
+Equations Build_t_OrZKPCommit {v_Z : _} {v_G : _} `{ t_Sized (v_Z)} `{ t_Sized (v_G)} `{ t_Z_Field (v_Z)} `{ t_Group (v_G) (v_Z)} {f_or_zkp_x : both0 (f_group_type)} {f_or_zkp_y : both0 (f_group_type)} {f_or_zkp_a1 : both0 (f_group_type)} {f_or_zkp_b1 : both0 (f_group_type)} {f_or_zkp_a2 : both0 (f_group_type)} {f_or_zkp_b2 : both0 (f_group_type)} {f_or_zkp_c : both0 (f_field_type)} {f_or_zkp_d1 : both0 (f_field_type)} {f_or_zkp_d2 : both0 (f_field_type)} {f_or_zkp_r1 : both0 (f_field_type)} {f_or_zkp_r2 : both0 (f_field_type)} : both0 (t_OrZKPCommit) :=
   Build_t_OrZKPCommit  :=
     bind_both f_or_zkp_r2 (fun f_or_zkp_r2 =>
       bind_both f_or_zkp_r1 (fun f_or_zkp_r1 =>
@@ -188,7 +235,7 @@ Equations Build_t_OrZKPCommit {v_Z : _} {v_G : _} `{ t_Sized (v_Z)} `{ t_Sized (
                     bind_both f_or_zkp_a1 (fun f_or_zkp_a1 =>
                       bind_both f_or_zkp_y (fun f_or_zkp_y =>
                         bind_both f_or_zkp_x (fun f_or_zkp_x =>
-                          solve_lift (ret_both ((f_or_zkp_x,f_or_zkp_y,f_or_zkp_a1,f_or_zkp_b1,f_or_zkp_a2,f_or_zkp_b2,f_or_zkp_c,f_or_zkp_d1,f_or_zkp_d2,f_or_zkp_r1,f_or_zkp_r2) : (t_OrZKPCommit)))))))))))))) : both (t_OrZKPCommit).
+                          solve_lift (ret_both ((f_or_zkp_x,f_or_zkp_y,f_or_zkp_a1,f_or_zkp_b1,f_or_zkp_a2,f_or_zkp_b2,f_or_zkp_c,f_or_zkp_d1,f_or_zkp_d2,f_or_zkp_r1,f_or_zkp_r2) : (t_OrZKPCommit)))))))))))))) : both0 (t_OrZKPCommit).
 Fail Next Obligation.
 Notation "'Build_t_OrZKPCommit' '[' x ']' '(' 'f_or_zkp_x' ':=' y ')'" := (Build_t_OrZKPCommit (f_or_zkp_x := y) (f_or_zkp_y := f_or_zkp_y x) (f_or_zkp_a1 := f_or_zkp_a1 x) (f_or_zkp_b1 := f_or_zkp_b1 x) (f_or_zkp_a2 := f_or_zkp_a2 x) (f_or_zkp_b2 := f_or_zkp_b2 x) (f_or_zkp_c := f_or_zkp_c x) (f_or_zkp_d1 := f_or_zkp_d1 x) (f_or_zkp_d2 := f_or_zkp_d2 x) (f_or_zkp_r1 := f_or_zkp_r1 x) (f_or_zkp_r2 := f_or_zkp_r2 x)).
 Notation "'Build_t_OrZKPCommit' '[' x ']' '(' 'f_or_zkp_y' ':=' y ')'" := (Build_t_OrZKPCommit (f_or_zkp_x := f_or_zkp_x x) (f_or_zkp_y := y) (f_or_zkp_a1 := f_or_zkp_a1 x) (f_or_zkp_b1 := f_or_zkp_b1 x) (f_or_zkp_a2 := f_or_zkp_a2 x) (f_or_zkp_b2 := f_or_zkp_b2 x) (f_or_zkp_c := f_or_zkp_c x) (f_or_zkp_d1 := f_or_zkp_d1 x) (f_or_zkp_d2 := f_or_zkp_d2 x) (f_or_zkp_r1 := f_or_zkp_r1 x) (f_or_zkp_r2 := f_or_zkp_r2 x)).
@@ -204,27 +251,27 @@ Notation "'Build_t_OrZKPCommit' '[' x ']' '(' 'f_or_zkp_r2' ':=' y ')'" := (Buil
 
 Definition t_RegisterParam {v_Z : _} `{ t_Sized (v_Z)} `{ t_Z_Field (v_Z)} : choice_type :=
   (int32 × f_field_type × int32).
-Equations f_rp_i {v_Z : _} `{ t_Sized (v_Z)} `{ t_Z_Field (v_Z)} (s : both (t_RegisterParam)) : both (int32) :=
+Equations f_rp_i {v_Z : _} `{ t_Sized (v_Z)} `{ t_Z_Field (v_Z)} (s : both0 (t_RegisterParam)) : both0 (int32) :=
   f_rp_i s  :=
     bind_both s (fun x =>
-      solve_lift (ret_both (fst (fst x) : int32))) : both (int32).
+      solve_lift (ret_both (fst (fst x) : int32))) : both0 (int32).
 Fail Next Obligation.
-Equations f_rp_xi {v_Z : _} `{ t_Sized (v_Z)} `{ t_Z_Field (v_Z)} (s : both (t_RegisterParam)) : both (f_field_type) :=
+Equations f_rp_xi {v_Z : _} `{ t_Sized (v_Z)} `{ t_Z_Field (v_Z)} (s : both0 (t_RegisterParam)) : both0 (f_field_type) :=
   f_rp_xi s  :=
     bind_both s (fun x =>
-      solve_lift (ret_both (snd (fst x) : f_field_type))) : both (f_field_type).
+      solve_lift (ret_both (snd (fst x) : f_field_type))) : both0 (f_field_type).
 Fail Next Obligation.
-Equations f_rp_zkp_random {v_Z : _} `{ t_Sized (v_Z)} `{ t_Z_Field (v_Z)} (s : both (t_RegisterParam)) : both (int32) :=
+Equations f_rp_zkp_random {v_Z : _} `{ t_Sized (v_Z)} `{ t_Z_Field (v_Z)} (s : both0 (t_RegisterParam)) : both0 (int32) :=
   f_rp_zkp_random s  :=
     bind_both s (fun x =>
-      solve_lift (ret_both (snd x : int32))) : both (int32).
+      solve_lift (ret_both (snd x : int32))) : both0 (int32).
 Fail Next Obligation.
-Equations Build_t_RegisterParam {v_Z : _} `{ t_Sized (v_Z)} `{ t_Z_Field (v_Z)} {f_rp_i : both (int32)} {f_rp_xi : both (f_field_type)} {f_rp_zkp_random : both (int32)} : both (t_RegisterParam) :=
+Equations Build_t_RegisterParam {v_Z : _} `{ t_Sized (v_Z)} `{ t_Z_Field (v_Z)} {f_rp_i : both0 (int32)} {f_rp_xi : both0 (f_field_type)} {f_rp_zkp_random : both0 (int32)} : both0 (t_RegisterParam) :=
   Build_t_RegisterParam  :=
     bind_both f_rp_zkp_random (fun f_rp_zkp_random =>
       bind_both f_rp_xi (fun f_rp_xi =>
         bind_both f_rp_i (fun f_rp_i =>
-          solve_lift (ret_both ((f_rp_i,f_rp_xi,f_rp_zkp_random) : (t_RegisterParam)))))) : both (t_RegisterParam).
+          solve_lift (ret_both ((f_rp_i,f_rp_xi,f_rp_zkp_random) : (t_RegisterParam)))))) : both0 (t_RegisterParam).
 Fail Next Obligation.
 Notation "'Build_t_RegisterParam' '[' x ']' '(' 'f_rp_i' ':=' y ')'" := (Build_t_RegisterParam (f_rp_i := y) (f_rp_xi := f_rp_xi x) (f_rp_zkp_random := f_rp_zkp_random x)).
 Notation "'Build_t_RegisterParam' '[' x ']' '(' 'f_rp_xi' ':=' y ')'" := (Build_t_RegisterParam (f_rp_i := f_rp_i x) (f_rp_xi := y) (f_rp_zkp_random := f_rp_zkp_random x)).
@@ -232,27 +279,27 @@ Notation "'Build_t_RegisterParam' '[' x ']' '(' 'f_rp_zkp_random' ':=' y ')'" :=
 
 Definition t_SchnorrZKPCommit {v_Z : _} {v_G : _} `{ t_Sized (v_Z)} `{ t_Sized (v_G)} `{ t_Z_Field (v_Z)} `{ t_Group (v_G) (v_Z)} : choice_type :=
   (f_group_type × f_field_type × f_field_type).
-Equations f_schnorr_zkp_u {v_Z : _} {v_G : _} `{ t_Sized (v_Z)} `{ t_Sized (v_G)} `{ t_Z_Field (v_Z)} `{ t_Group (v_G) (v_Z)} (s : both (t_SchnorrZKPCommit)) : both (f_group_type) :=
+Equations f_schnorr_zkp_u {v_Z : _} {v_G : _} `{ t_Sized (v_Z)} `{ t_Sized (v_G)} `{ t_Z_Field (v_Z)} `{ t_Group (v_G) (v_Z)} (s : both0 (t_SchnorrZKPCommit)) : both0 (f_group_type) :=
   f_schnorr_zkp_u s  :=
     bind_both s (fun x =>
-      solve_lift (ret_both (fst (fst x) : f_group_type))) : both (f_group_type).
+      solve_lift (ret_both (fst (fst x) : f_group_type))) : both0 (f_group_type).
 Fail Next Obligation.
-Equations f_schnorr_zkp_c {v_Z : _} {v_G : _} `{ t_Sized (v_Z)} `{ t_Sized (v_G)} `{ t_Z_Field (v_Z)} `{ t_Group (v_G) (v_Z)} (s : both (t_SchnorrZKPCommit)) : both (f_field_type) :=
+Equations f_schnorr_zkp_c {v_Z : _} {v_G : _} `{ t_Sized (v_Z)} `{ t_Sized (v_G)} `{ t_Z_Field (v_Z)} `{ t_Group (v_G) (v_Z)} (s : both0 (t_SchnorrZKPCommit)) : both0 (f_field_type) :=
   f_schnorr_zkp_c s  :=
     bind_both s (fun x =>
-      solve_lift (ret_both (snd (fst x) : f_field_type))) : both (f_field_type).
+      solve_lift (ret_both (snd (fst x) : f_field_type))) : both0 (f_field_type).
 Fail Next Obligation.
-Equations f_schnorr_zkp_z {v_Z : _} {v_G : _} `{ t_Sized (v_Z)} `{ t_Sized (v_G)} `{ t_Z_Field (v_Z)} `{ t_Group (v_G) (v_Z)} (s : both (t_SchnorrZKPCommit)) : both (f_field_type) :=
+Equations f_schnorr_zkp_z {v_Z : _} {v_G : _} `{ t_Sized (v_Z)} `{ t_Sized (v_G)} `{ t_Z_Field (v_Z)} `{ t_Group (v_G) (v_Z)} (s : both0 (t_SchnorrZKPCommit)) : both0 (f_field_type) :=
   f_schnorr_zkp_z s  :=
     bind_both s (fun x =>
-      solve_lift (ret_both (snd x : f_field_type))) : both (f_field_type).
+      solve_lift (ret_both (snd x : f_field_type))) : both0 (f_field_type).
 Fail Next Obligation.
-Equations Build_t_SchnorrZKPCommit {v_Z : _} {v_G : _} `{ t_Sized (v_Z)} `{ t_Sized (v_G)} `{ t_Z_Field (v_Z)} `{ t_Group (v_G) (v_Z)} {f_schnorr_zkp_u : both (f_group_type)} {f_schnorr_zkp_c : both (f_field_type)} {f_schnorr_zkp_z : both (f_field_type)} : both (t_SchnorrZKPCommit) :=
+Equations Build_t_SchnorrZKPCommit {v_Z : _} {v_G : _} `{ t_Sized (v_Z)} `{ t_Sized (v_G)} `{ t_Z_Field (v_Z)} `{ t_Group (v_G) (v_Z)} {f_schnorr_zkp_u : both0 (f_group_type)} {f_schnorr_zkp_c : both0 (f_field_type)} {f_schnorr_zkp_z : both0 (f_field_type)} : both0 (t_SchnorrZKPCommit) :=
   Build_t_SchnorrZKPCommit  :=
     bind_both f_schnorr_zkp_z (fun f_schnorr_zkp_z =>
       bind_both f_schnorr_zkp_c (fun f_schnorr_zkp_c =>
         bind_both f_schnorr_zkp_u (fun f_schnorr_zkp_u =>
-          solve_lift (ret_both ((f_schnorr_zkp_u,f_schnorr_zkp_c,f_schnorr_zkp_z) : (t_SchnorrZKPCommit)))))) : both (t_SchnorrZKPCommit).
+          solve_lift (ret_both ((f_schnorr_zkp_u,f_schnorr_zkp_c,f_schnorr_zkp_z) : (t_SchnorrZKPCommit)))))) : both0 (t_SchnorrZKPCommit).
 Fail Next Obligation.
 Notation "'Build_t_SchnorrZKPCommit' '[' x ']' '(' 'f_schnorr_zkp_u' ':=' y ')'" := (Build_t_SchnorrZKPCommit (f_schnorr_zkp_u := y) (f_schnorr_zkp_c := f_schnorr_zkp_c x) (f_schnorr_zkp_z := f_schnorr_zkp_z x)).
 Notation "'Build_t_SchnorrZKPCommit' '[' x ']' '(' 'f_schnorr_zkp_c' ':=' y ')'" := (Build_t_SchnorrZKPCommit (f_schnorr_zkp_u := f_schnorr_zkp_u x) (f_schnorr_zkp_c := y) (f_schnorr_zkp_z := f_schnorr_zkp_z x)).
@@ -260,31 +307,31 @@ Notation "'Build_t_SchnorrZKPCommit' '[' x ']' '(' 'f_schnorr_zkp_z' ':=' y ')'"
 
 Definition t_TallyParameter : choice_type :=
   'unit.
-Equations Build_t_TallyParameter : both (t_TallyParameter) :=
+Equations Build_t_TallyParameter : both0 (t_TallyParameter) :=
   Build_t_TallyParameter  :=
-    solve_lift (ret_both (tt (* Empty tuple *) : (t_TallyParameter))) : both (t_TallyParameter).
+    solve_lift (ret_both (tt (* Empty tuple *) : (t_TallyParameter))) : both0 (t_TallyParameter).
 Fail Next Obligation.
 
-Equations schnorr_zkp {v_Z : _} {v_G : _} `{ t_Sized (v_Z)} `{ t_Sized (v_G)} `{ t_Z_Field (v_Z)} `{ t_Group (v_G) (v_Z)} (random : both (int32)) (h : both (f_group_type)) (x : both (f_field_type)) : both (t_SchnorrZKPCommit (v_Z := v_Z) (v_G := v_G)) :=
+Equations schnorr_zkp {v_Z : _} {v_G : _} `{ t_Sized (v_Z)} `{ t_Sized (v_G)} `{ t_Z_Field (v_Z)} `{ t_Group (v_G) (v_Z)} (random : both0 (int32)) (h : both0 (f_group_type)) (x : both0 (f_field_type)) : both0 (t_SchnorrZKPCommit (v_Z := v_Z) (v_G := v_G)) :=
   schnorr_zkp random h x  :=
     solve_lift (run (letb r := f_random_field_elem random in
     letb u := f_g_pow r in
-    letb c := f_hash (impl__into_vec (unsize (box_new (array_from_list [f_g (ret_both (tt : 'unit));
+    letb c := f_hash (impl__into_vec (unsize (box_new (array_from_list [f_g;
       h;
       u])))) in
     letb z := f_add r (f_mul c x) in
-    letm[choice_typeMonad.result_bind_code (t_SchnorrZKPCommit (v_Z := v_Z) (v_G := v_G))] hoist1 := v_Break (Build_t_SchnorrZKPCommit (f_schnorr_zkp_u := u) (f_schnorr_zkp_c := c) (f_schnorr_zkp_z := z)) in
-    ControlFlow_Continue (never_to_any hoist1))) : both (t_SchnorrZKPCommit (v_Z := v_Z) (v_G := v_G)).
+    letm[choice_typeMonad.result_bind_code (t_SchnorrZKPCommit (v_Z := v_Z) (v_G := v_G))] hoist1 := _ (* v_Break (Build_t_SchnorrZKPCommit (f_schnorr_zkp_u := u) (f_schnorr_zkp_c := c) (f_schnorr_zkp_z := z)) *) in
+    ControlFlow_Continue _ (* (never_to_any hoist1) *))) : both0 (t_SchnorrZKPCommit (v_Z := v_Z) (v_G := v_G)).
 Fail Next Obligation.
 
-Equations schnorr_zkp_validate {v_Z : _} {v_G : _} `{ t_Sized (v_Z)} `{ t_Sized (v_G)} `{ t_Z_Field (v_Z)} `{ t_Group (v_G) (v_Z)} (h : both (f_group_type)) (pi : both (t_SchnorrZKPCommit (v_Z := v_Z) (v_G := v_G))) : both ('bool) :=
+Equations schnorr_zkp_validate {v_Z : _} {v_G : _} `{ t_Sized (v_Z)} `{ t_Sized (v_G)} `{ t_Z_Field (v_Z)} `{ t_Group (v_G) (v_Z)} (h : both0 (f_group_type)) (pi : both0 (t_SchnorrZKPCommit (v_Z := v_Z) (v_G := v_G))) : both0 ('bool) :=
   schnorr_zkp_validate h pi  :=
     solve_lift (andb ((f_schnorr_zkp_c pi) =.? (f_hash (impl__into_vec (unsize (box_new (array_from_list [f_g (ret_both (tt : 'unit));
       h;
-      f_schnorr_zkp_u pi])))))) ((f_g_pow (f_schnorr_zkp_z pi)) =.? (f_prod (f_schnorr_zkp_u pi) (f_pow h (f_schnorr_zkp_c pi))))) : both ('bool).
+      f_schnorr_zkp_u pi])))))) ((f_g_pow (f_schnorr_zkp_z pi)) =.? (f_prod (f_schnorr_zkp_u pi) (f_pow h (f_schnorr_zkp_c pi))))) : both0 ('bool).
 Fail Next Obligation.
 
-Equations zkp_one_out_of_two {v_Z : _} {v_G : _} `{ t_Sized (v_Z)} `{ t_Sized (v_G)} `{ t_Z_Field (v_Z)} `{ t_Group (v_G) (v_Z)} (random_w : both (int32)) (random_r : both (int32)) (random_d : both (int32)) (h : both (f_group_type)) (xi : both (f_field_type)) (vi : both ('bool)) : both (t_OrZKPCommit (v_Z := v_Z) (v_G := v_G)) :=
+Equations zkp_one_out_of_two {v_Z : _} {v_G : _} `{ t_Sized (v_Z)} `{ t_Sized (v_G)} `{ t_Z_Field (v_Z)} `{ t_Group (v_G) (v_Z)} (random_w : both0 (int32)) (random_r : both0 (int32)) (random_d : both0 (int32)) (h : both0 (f_group_type)) (xi : both0 (f_field_type)) (vi : both0 ('bool)) : both0 (t_OrZKPCommit (v_Z := v_Z) (v_G := v_G)) :=
   zkp_one_out_of_two random_w random_r random_d h xi vi  :=
     letb w := f_random_field_elem random_w in
     solve_lift (ifb vi
@@ -321,10 +368,10 @@ Equations zkp_one_out_of_two {v_Z : _} {v_G : _} `{ t_Sized (v_Z)} `{ t_Sized (v
       b2])))) in
     letb d1 := f_sub c d2 in
     letb r1 := f_sub w (f_mul xi d1) in
-    Build_t_OrZKPCommit (f_or_zkp_x := x) (f_or_zkp_y := y) (f_or_zkp_a1 := a1) (f_or_zkp_b1 := b1) (f_or_zkp_a2 := a2) (f_or_zkp_b2 := b2) (f_or_zkp_c := c) (f_or_zkp_d1 := d1) (f_or_zkp_d2 := d2) (f_or_zkp_r1 := r1) (f_or_zkp_r2 := r2)) : both (t_OrZKPCommit (v_Z := v_Z) (v_G := v_G)).
+    Build_t_OrZKPCommit (f_or_zkp_x := x) (f_or_zkp_y := y) (f_or_zkp_a1 := a1) (f_or_zkp_b1 := b1) (f_or_zkp_a2 := a2) (f_or_zkp_b2 := b2) (f_or_zkp_c := c) (f_or_zkp_d1 := d1) (f_or_zkp_d2 := d2) (f_or_zkp_r1 := r1) (f_or_zkp_r2 := r2)) : both0 (t_OrZKPCommit (v_Z := v_Z) (v_G := v_G)).
 Fail Next Obligation.
 
-Equations zkp_one_out_of_two_validate {v_Z : _} {v_G : _} `{ t_Sized (v_Z)} `{ t_Sized (v_G)} `{ t_Z_Field (v_Z)} `{ t_Group (v_G) (v_Z)} (h : both (f_group_type)) (zkp : both (t_OrZKPCommit (v_Z := v_Z) (v_G := v_G))) : both ('bool) :=
+Equations zkp_one_out_of_two_validate {v_Z : _} {v_G : _} `{ t_Sized (v_Z)} `{ t_Sized (v_G)} `{ t_Z_Field (v_Z)} `{ t_Group (v_G) (v_Z)} (h : both0 (f_group_type)) (zkp : both0 (t_OrZKPCommit (v_Z := v_Z) (v_G := v_G))) : both0 ('bool) :=
   zkp_one_out_of_two_validate h zkp  :=
     letb c := f_hash (impl__into_vec (unsize (box_new (array_from_list [f_or_zkp_x zkp;
       f_or_zkp_y zkp;
@@ -332,42 +379,42 @@ Equations zkp_one_out_of_two_validate {v_Z : _} {v_G : _} `{ t_Sized (v_Z)} `{ t
       f_or_zkp_b1 zkp;
       f_or_zkp_a2 zkp;
       f_or_zkp_b2 zkp])))) in
-    solve_lift (andb (andb (andb (andb (c =.? (f_add (f_or_zkp_d1 zkp) (f_or_zkp_d2 zkp))) ((f_or_zkp_a1 zkp) =.? (f_prod (f_g_pow (f_or_zkp_r1 zkp)) (f_pow (f_or_zkp_x zkp) (f_or_zkp_d1 zkp))))) ((f_or_zkp_b1 zkp) =.? (f_prod (f_pow h (f_or_zkp_r1 zkp)) (f_pow (f_or_zkp_y zkp) (f_or_zkp_d1 zkp))))) ((f_or_zkp_a2 zkp) =.? (f_prod (f_g_pow (f_or_zkp_r2 zkp)) (f_pow (f_or_zkp_x zkp) (f_or_zkp_d2 zkp))))) ((f_or_zkp_b2 zkp) =.? (f_prod (f_pow h (f_or_zkp_r2 zkp)) (f_pow (f_div (f_or_zkp_y zkp) (f_g (ret_both (tt : 'unit)))) (f_or_zkp_d2 zkp))))) : both ('bool).
+    solve_lift (andb (andb (andb (andb (c =.? (f_add (f_or_zkp_d1 zkp) (f_or_zkp_d2 zkp))) ((f_or_zkp_a1 zkp) =.? (f_prod (f_g_pow (f_or_zkp_r1 zkp)) (f_pow (f_or_zkp_x zkp) (f_or_zkp_d1 zkp))))) ((f_or_zkp_b1 zkp) =.? (f_prod (f_pow h (f_or_zkp_r1 zkp)) (f_pow (f_or_zkp_y zkp) (f_or_zkp_d1 zkp))))) ((f_or_zkp_a2 zkp) =.? (f_prod (f_g_pow (f_or_zkp_r2 zkp)) (f_pow (f_or_zkp_x zkp) (f_or_zkp_d2 zkp))))) ((f_or_zkp_b2 zkp) =.? (f_prod (f_pow h (f_or_zkp_r2 zkp)) (f_pow (f_div (f_or_zkp_y zkp) (f_g (ret_both (tt : 'unit)))) (f_or_zkp_d2 zkp))))) : both0 ('bool).
 Fail Next Obligation.
 
-Definition t_OvnContractState {v_Z : _} {v_G : _} {n : both (uint_size)} `{ t_Sized (v_Z)} `{ t_Sized (v_G)} `{ t_Z_Field (v_Z)} `{ t_Group (v_G) (v_Z)} : choice_type :=
+Definition t_OvnContractState {v_Z : _} {v_G : _} {n : both0 (uint_size)} `{ t_Sized (v_Z)} `{ t_Sized (v_G)} `{ t_Z_Field (v_Z)} `{ t_Group (v_G) (v_Z)} : choice_type :=
   (nseq f_group_type (is_pure (n)) × nseq (t_SchnorrZKPCommit (v_Z := v_Z) (v_G := v_G)) (is_pure (n)) × nseq f_field_type (is_pure (n)) × nseq f_group_type (is_pure (n)) × nseq (t_OrZKPCommit (v_Z := v_Z) (v_G := v_G)) (is_pure (n)) × int32).
-Equations f_g_pow_xis {v_Z : _} {v_G : _} {n : both (uint_size)} `{ t_Sized (v_Z)} `{ t_Sized (v_G)} `{ t_Z_Field (v_Z)} `{ t_Group (v_G) (v_Z)} (s : both (t_OvnContractState (n := n))) : both (nseq f_group_type (is_pure (n))) :=
+Equations f_g_pow_xis {v_Z : _} {v_G : _} {n : both0 (uint_size)} `{ t_Sized (v_Z)} `{ t_Sized (v_G)} `{ t_Z_Field (v_Z)} `{ t_Group (v_G) (v_Z)} (s : both0 (t_OvnContractState (n := n))) : both0 (nseq f_group_type (is_pure (n))) :=
   f_g_pow_xis s  :=
     bind_both s (fun x =>
-      solve_lift (ret_both (fst (fst (fst (fst (fst x)))) : nseq f_group_type (is_pure (n))))) : both (nseq f_group_type (is_pure (n))).
+      solve_lift (ret_both (fst (fst (fst (fst (fst x)))) : nseq f_group_type (is_pure (n))))) : both0 (nseq f_group_type (is_pure (n))).
 Fail Next Obligation.
-Equations f_zkp_xis {v_Z : _} {v_G : _} {n : both (uint_size)} `{ t_Sized (v_Z)} `{ t_Sized (v_G)} `{ t_Z_Field (v_Z)} `{ t_Group (v_G) (v_Z)} (s : both (t_OvnContractState (n := n))) : both (nseq (t_SchnorrZKPCommit (v_Z := v_Z) (v_G := v_G)) (is_pure (n))) :=
+Equations f_zkp_xis {v_Z : _} {v_G : _} {n : both0 (uint_size)} `{ t_Sized (v_Z)} `{ t_Sized (v_G)} `{ t_Z_Field (v_Z)} `{ t_Group (v_G) (v_Z)} (s : both0 (t_OvnContractState (n := n))) : both0 (nseq (t_SchnorrZKPCommit (v_Z := v_Z) (v_G := v_G)) (is_pure (n))) :=
   f_zkp_xis s  :=
     bind_both s (fun x =>
-      solve_lift (ret_both (snd (fst (fst (fst (fst x)))) : nseq (t_SchnorrZKPCommit (v_Z := v_Z) (v_G := v_G)) (is_pure (n))))) : both (nseq (t_SchnorrZKPCommit (v_Z := v_Z) (v_G := v_G)) (is_pure (n))).
+      solve_lift (ret_both (snd (fst (fst (fst (fst x)))) : nseq (t_SchnorrZKPCommit (v_Z := v_Z) (v_G := v_G)) (is_pure (n))))) : both0 (nseq (t_SchnorrZKPCommit (v_Z := v_Z) (v_G := v_G)) (is_pure (n))).
 Fail Next Obligation.
-Equations f_commit_vis {v_Z : _} {v_G : _} {n : both (uint_size)} `{ t_Sized (v_Z)} `{ t_Sized (v_G)} `{ t_Z_Field (v_Z)} `{ t_Group (v_G) (v_Z)} (s : both (t_OvnContractState (n := n))) : both (nseq f_field_type (is_pure (n))) :=
+Equations f_commit_vis {v_Z : _} {v_G : _} {n : both0 (uint_size)} `{ t_Sized (v_Z)} `{ t_Sized (v_G)} `{ t_Z_Field (v_Z)} `{ t_Group (v_G) (v_Z)} (s : both0 (t_OvnContractState (n := n))) : both0 (nseq f_field_type (is_pure (n))) :=
   f_commit_vis s  :=
     bind_both s (fun x =>
-      solve_lift (ret_both (snd (fst (fst (fst x))) : nseq f_field_type (is_pure (n))))) : both (nseq f_field_type (is_pure (n))).
+      solve_lift (ret_both (snd (fst (fst (fst x))) : nseq f_field_type (is_pure (n))))) : both0 (nseq f_field_type (is_pure (n))).
 Fail Next Obligation.
-Equations f_g_pow_xi_yi_vis {v_Z : _} {v_G : _} {n : both (uint_size)} `{ t_Sized (v_Z)} `{ t_Sized (v_G)} `{ t_Z_Field (v_Z)} `{ t_Group (v_G) (v_Z)} (s : both (t_OvnContractState (n := n))) : both (nseq f_group_type (is_pure (n))) :=
+Equations f_g_pow_xi_yi_vis {v_Z : _} {v_G : _} {n : both0 (uint_size)} `{ t_Sized (v_Z)} `{ t_Sized (v_G)} `{ t_Z_Field (v_Z)} `{ t_Group (v_G) (v_Z)} (s : both0 (t_OvnContractState (n := n))) : both0 (nseq f_group_type (is_pure (n))) :=
   f_g_pow_xi_yi_vis s  :=
     bind_both s (fun x =>
-      solve_lift (ret_both (snd (fst (fst x)) : nseq f_group_type (is_pure (n))))) : both (nseq f_group_type (is_pure (n))).
+      solve_lift (ret_both (snd (fst (fst x)) : nseq f_group_type (is_pure (n))))) : both0 (nseq f_group_type (is_pure (n))).
 Fail Next Obligation.
-Equations f_zkp_vis {v_Z : _} {v_G : _} {n : both (uint_size)} `{ t_Sized (v_Z)} `{ t_Sized (v_G)} `{ t_Z_Field (v_Z)} `{ t_Group (v_G) (v_Z)} (s : both (t_OvnContractState (n := n))) : both (nseq (t_OrZKPCommit (v_Z := v_Z) (v_G := v_G)) (is_pure (n))) :=
+Equations f_zkp_vis {v_Z : _} {v_G : _} {n : both0 (uint_size)} `{ t_Sized (v_Z)} `{ t_Sized (v_G)} `{ t_Z_Field (v_Z)} `{ t_Group (v_G) (v_Z)} (s : both0 (t_OvnContractState (n := n))) : both0 (nseq (t_OrZKPCommit (v_Z := v_Z) (v_G := v_G)) (is_pure (n))) :=
   f_zkp_vis s  :=
     bind_both s (fun x =>
-      solve_lift (ret_both (snd (fst x) : nseq (t_OrZKPCommit (v_Z := v_Z) (v_G := v_G)) (is_pure (n))))) : both (nseq (t_OrZKPCommit (v_Z := v_Z) (v_G := v_G)) (is_pure (n))).
+      solve_lift (ret_both (snd (fst x) : nseq (t_OrZKPCommit (v_Z := v_Z) (v_G := v_G)) (is_pure (n))))) : both0 (nseq (t_OrZKPCommit (v_Z := v_Z) (v_G := v_G)) (is_pure (n))).
 Fail Next Obligation.
-Equations f_tally {v_Z : _} {v_G : _} {n : both (uint_size)} `{ t_Sized (v_Z)} `{ t_Sized (v_G)} `{ t_Z_Field (v_Z)} `{ t_Group (v_G) (v_Z)} (s : both (t_OvnContractState (n := n))) : both (int32) :=
+Equations f_tally {v_Z : _} {v_G : _} {n : both0 (uint_size)} `{ t_Sized (v_Z)} `{ t_Sized (v_G)} `{ t_Z_Field (v_Z)} `{ t_Group (v_G) (v_Z)} (s : both0 (t_OvnContractState (n := n))) : both0 (int32) :=
   f_tally s  :=
     bind_both s (fun x =>
-      solve_lift (ret_both (snd x : int32))) : both (int32).
+      solve_lift (ret_both (snd x : int32))) : both0 (int32).
 Fail Next Obligation.
-Equations Build_t_OvnContractState {v_Z : _} {v_G : _} {n : both (uint_size)} `{ t_Sized (v_Z)} `{ t_Sized (v_G)} `{ t_Z_Field (v_Z)} `{ t_Group (v_G) (v_Z)} {f_g_pow_xis : both (nseq f_group_type (is_pure (n)))} {f_zkp_xis : both (nseq (t_SchnorrZKPCommit (v_Z := v_Z) (v_G := v_G)) (is_pure (n)))} {f_commit_vis : both (nseq f_field_type (is_pure (n)))} {f_g_pow_xi_yi_vis : both (nseq f_group_type (is_pure (n)))} {f_zkp_vis : both (nseq (t_OrZKPCommit (v_Z := v_Z) (v_G := v_G)) (is_pure (n)))} {f_tally : both (int32)} : both (t_OvnContractState (n := n)) :=
+Equations Build_t_OvnContractState {v_Z : _} {v_G : _} {n : both0 (uint_size)} `{ t_Sized (v_Z)} `{ t_Sized (v_G)} `{ t_Z_Field (v_Z)} `{ t_Group (v_G) (v_Z)} {f_g_pow_xis : both0 (nseq f_group_type (is_pure (n)))} {f_zkp_xis : both0 (nseq (t_SchnorrZKPCommit (v_Z := v_Z) (v_G := v_G)) (is_pure (n)))} {f_commit_vis : both0 (nseq f_field_type (is_pure (n)))} {f_g_pow_xi_yi_vis : both0 (nseq f_group_type (is_pure (n)))} {f_zkp_vis : both0 (nseq (t_OrZKPCommit (v_Z := v_Z) (v_G := v_G)) (is_pure (n)))} {f_tally : both0 (int32)} : both0 (t_OvnContractState (n := n)) :=
   Build_t_OvnContractState  :=
     bind_both f_tally (fun f_tally =>
       bind_both f_zkp_vis (fun f_zkp_vis =>
@@ -375,7 +422,7 @@ Equations Build_t_OvnContractState {v_Z : _} {v_G : _} {n : both (uint_size)} `{
           bind_both f_commit_vis (fun f_commit_vis =>
             bind_both f_zkp_xis (fun f_zkp_xis =>
               bind_both f_g_pow_xis (fun f_g_pow_xis =>
-                solve_lift (ret_both ((f_g_pow_xis,f_zkp_xis,f_commit_vis,f_g_pow_xi_yi_vis,f_zkp_vis,f_tally) : (t_OvnContractState))))))))) : both (t_OvnContractState).
+                solve_lift (ret_both ((f_g_pow_xis,f_zkp_xis,f_commit_vis,f_g_pow_xi_yi_vis,f_zkp_vis,f_tally) : (t_OvnContractState))))))))) : both0 (t_OvnContractState).
 Fail Next Obligation.
 Notation "'Build_t_OvnContractState' '[' x ']' '(' 'f_g_pow_xis' ':=' y ')'" := (Build_t_OvnContractState (f_g_pow_xis := y) (f_zkp_xis := f_zkp_xis x) (f_commit_vis := f_commit_vis x) (f_g_pow_xi_yi_vis := f_g_pow_xi_yi_vis x) (f_zkp_vis := f_zkp_vis x) (f_tally := f_tally x)).
 Notation "'Build_t_OvnContractState' '[' x ']' '(' 'f_zkp_xis' ':=' y ')'" := (Build_t_OvnContractState (f_g_pow_xis := f_g_pow_xis x) (f_zkp_xis := y) (f_commit_vis := f_commit_vis x) (f_g_pow_xi_yi_vis := f_g_pow_xi_yi_vis x) (f_zkp_vis := f_zkp_vis x) (f_tally := f_tally x)).
@@ -384,7 +431,7 @@ Notation "'Build_t_OvnContractState' '[' x ']' '(' 'f_g_pow_xi_yi_vis' ':=' y ')
 Notation "'Build_t_OvnContractState' '[' x ']' '(' 'f_zkp_vis' ':=' y ')'" := (Build_t_OvnContractState (f_g_pow_xis := f_g_pow_xis x) (f_zkp_xis := f_zkp_xis x) (f_commit_vis := f_commit_vis x) (f_g_pow_xi_yi_vis := f_g_pow_xi_yi_vis x) (f_zkp_vis := y) (f_tally := f_tally x)).
 Notation "'Build_t_OvnContractState' '[' x ']' '(' 'f_tally' ':=' y ')'" := (Build_t_OvnContractState (f_g_pow_xis := f_g_pow_xis x) (f_zkp_xis := f_zkp_xis x) (f_commit_vis := f_commit_vis x) (f_g_pow_xi_yi_vis := f_g_pow_xi_yi_vis x) (f_zkp_vis := f_zkp_vis x) (f_tally := y)).
 
-Equations cast_vote {v_Z : _} {v_G : _} {n : both (uint_size)} {v_A : _} {impl_574521470_ : _} `{ t_Sized (v_Z)} `{ t_Sized (v_G)} `{ t_Sized (v_A)} `{ t_Sized (impl_574521470_)} `{ t_Z_Field (v_Z)} `{ t_Group (v_G) (v_Z)} `{ t_HasActions (v_A)} `{ t_HasReceiveContext (impl_574521470_) ('unit)} (ctx : both (impl_574521470_)) (state : both (t_OvnContractState (v_Z := v_Z) (v_G := v_G) (n := n))) : both (t_Result ((v_A × t_OvnContractState (v_Z := v_Z) (v_G := v_G) (n := n))) (t_ParseError)) :=
+Equations cast_vote {v_Z : _} {v_G : _} {n : both0 (uint_size)} {v_A : _} {impl_574521470_ : _} `{ t_Sized (v_Z)} `{ t_Sized (v_G)} `{ t_Sized (v_A)} `{ t_Sized (impl_574521470_)} `{ t_Z_Field (v_Z)} `{ t_Group (v_G) (v_Z)} `{ t_HasActions (v_A)} `{ t_HasReceiveContext (impl_574521470_) ('unit)} (ctx : both0 (impl_574521470_)) (state : both0 (t_OvnContractState (v_Z := v_Z) (v_G := v_G) (n := n))) : both0 (t_Result ((v_A × t_OvnContractState (v_Z := v_Z) (v_G := v_G) (n := n))) (t_ParseError)) :=
   cast_vote ctx state  :=
     solve_lift (run (letb '(_,out) := f_get (f_parameter_cursor ctx) in
     letm[choice_typeMonad.result_bind_code (t_Result ((v_A × t_OvnContractState (v_Z := v_Z) (v_G := v_G) (n := n))) (t_ParseError))] (params : t_CastVoteParam (v_Z)) := matchb out with
@@ -402,10 +449,10 @@ Equations cast_vote {v_Z : _} {v_G : _} {n : both (uint_size)} {v_A : _} {impl_5
     letb cast_vote_state_ret := f_clone state in
     letb cast_vote_state_ret := Build_t_OvnContractState[cast_vote_state_ret] (f_g_pow_xi_yi_vis := update_at_usize (f_g_pow_xi_yi_vis cast_vote_state_ret) (cast_int (WS2 := _) (f_cvp_i params)) g_pow_xi_yi_vi) in
     letb cast_vote_state_ret := Build_t_OvnContractState[cast_vote_state_ret] (f_zkp_vis := update_at_usize (f_zkp_vis cast_vote_state_ret) (cast_int (WS2 := _) (f_cvp_i params)) zkp_vi) in
-    Result_Ok (prod_b (f_accept (* (ret_both (tt : 'unit)) *),cast_vote_state_ret))))) : both (t_Result ((v_A × t_OvnContractState (v_Z := v_Z) (v_G := v_G) (n := n))) (t_ParseError)).
+    Result_Ok (prod_b (f_accept (* (ret_both (tt : 'unit)) *),cast_vote_state_ret))))) : both0 (t_Result ((v_A × t_OvnContractState (v_Z := v_Z) (v_G := v_G) (n := n))) (t_ParseError)).
 Fail Next Obligation.
 
-Equations commit_to_vote {v_Z : _} {v_G : _} {n : both (uint_size)} {v_A : _} {impl_574521470_ : _} `{ t_Sized (v_Z)} `{ t_Sized (v_G)} `{ t_Sized (v_A)} `{ t_Sized (impl_574521470_)} `{ t_Z_Field (v_Z)} `{ t_Group (v_G) (v_Z)} `{ t_HasActions (v_A)} `{ t_HasReceiveContext (impl_574521470_) ('unit)} (ctx : both (impl_574521470_)) (state : both (t_OvnContractState (v_Z := v_Z) (v_G := v_G) (n := n))) : both (t_Result ((v_A × t_OvnContractState (v_Z := v_Z) (v_G := v_G) (n := n))) (t_ParseError)) :=
+Equations commit_to_vote {v_Z : _} {v_G : _} {n : both0 (uint_size)} {v_A : _} {impl_574521470_ : _} `{ t_Sized (v_Z)} `{ t_Sized (v_G)} `{ t_Sized (v_A)} `{ t_Sized (impl_574521470_)} `{ t_Z_Field (v_Z)} `{ t_Group (v_G) (v_Z)} `{ t_HasActions (v_A)} `{ t_HasReceiveContext (impl_574521470_) ('unit)} (ctx : both0 (impl_574521470_)) (state : both0 (t_OvnContractState (v_Z := v_Z) (v_G := v_G) (n := n))) : both0 (t_Result ((v_A × t_OvnContractState (v_Z := v_Z) (v_G := v_G) (n := n))) (t_ParseError)) :=
   commit_to_vote ctx state  :=
     solve_lift (run (letb '(_,out) := f_get (f_parameter_cursor ctx) in
     letm[choice_typeMonad.result_bind_code (t_Result ((v_A × t_OvnContractState (v_Z := v_Z) (v_G := v_G) (n := n))) (t_ParseError))] (params : t_CastVoteParam (v_Z)) := matchb out with
@@ -417,27 +464,27 @@ Equations commit_to_vote {v_Z : _} {v_G : _} {n : both (uint_size)} {v_A : _} {i
       letm[choice_typeMonad.result_bind_code (t_Result ((v_A × t_OvnContractState (v_Z := v_Z) (v_G := v_G) (n := n))) (t_ParseError))] hoist3 := v_Break (Result_Err (ret_both tt)) in
       ControlFlow_Continue (solve_lift (never_to_any hoist3))
     end in
-    ControlFlow_Continue (letb _ := foldi_both_list (f_into_iter (Build_t_Range (f_start := ret_both (0 : uint_size)) (f_end := n))) (fun i =>
+    ControlFlow_Continue (letb _ := foldi_both0_list (f_into_iter (Build_t_Range (f_start := ret_both (0 : uint_size)) (f_end := n))) (fun i =>
       ssp (fun _ =>
         solve_lift (ifb negb (schnorr_zkp_validate ((f_g_pow_xis state).a[i]) ((f_zkp_xis state).a[i]))
         then letm[choice_typeMonad.result_bind_code (t_Result ((v_A × t_OvnContractState (v_Z := v_Z) (v_G := v_G) (n := n))) (t_ParseError))] hoist4 := v_Break (Result_Err (ret_both tt)) in
         ControlFlow_Continue (never_to_any hoist4)
-        else ControlFlow_Continue (ret_both (tt : 'unit))) : both _ (* (t_ControlFlow (t_Result ((v_A × t_OvnContractState (v_Z := v_Z) (v_G := v_G) (n := n))) (t_ParseError)) ('unit)) *))) (Ok (ret_both (tt : 'unit))) in
+        else ControlFlow_Continue (ret_both (tt : 'unit))) : both0 _ (* (t_ControlFlow (t_Result ((v_A × t_OvnContractState (v_Z := v_Z) (v_G := v_G) (n := n))) (t_ParseError)) ('unit)) *))) (Ok (ret_both (tt : 'unit))) in
     letb g_pow_yi := compute_g_pow_yi (cast_int (WS2 := _) (f_cvp_i params)) (f_g_pow_xis state) in
     letb g_pow_xi_yi_vi := compute_group_element_for_vote (f_cvp_xi params) (f_cvp_vote params) g_pow_yi in
     letb commit_vi := commit_to g_pow_xi_yi_vi in
     letb commit_to_vote_state_ret := f_clone state in
     letb commit_to_vote_state_ret := Build_t_OvnContractState[commit_to_vote_state_ret] (f_commit_vis := update_at_usize (f_commit_vis commit_to_vote_state_ret) (cast_int (WS2 := _) (f_cvp_i params)) commit_vi) in
-                            Result_Ok (prod_b (f_accept (* (ret_both (tt : 'unit)) *),commit_to_vote_state_ret))))) : both (t_Result ((v_A × t_OvnContractState (v_Z := v_Z) (v_G := v_G) (n := n))) (t_ParseError)).
+                            Result_Ok (prod_b (f_accept (* (ret_both (tt : 'unit)) *),commit_to_vote_state_ret))))) : both0 (t_Result ((v_A × t_OvnContractState (v_Z := v_Z) (v_G := v_G) (n := n))) (t_ParseError)).
 Solve All Obligations with now intros ; destruct from_uint_size.
 Fail Next Obligation.
 
-Equations init_ovn_contract {v_Z : _} {v_G : _} {n : both (uint_size)} `{ t_Sized (v_Z)} `{ t_Sized (v_G)} `{ t_Z_Field (v_Z)} `{ t_Group (v_G) (v_Z)} (_ : both ('unit)) : both (t_Result (t_OvnContractState (v_Z := v_Z) (v_G := v_G) (n := n)) (t_Reject)) :=
+Equations init_ovn_contract {v_Z : _} {v_G : _} {n : both0 (uint_size)} `{ t_Sized (v_Z)} `{ t_Sized (v_G)} `{ t_Z_Field (v_Z)} `{ t_Group (v_G) (v_Z)} (_ : both0 ('unit)) : both0 (t_Result (t_OvnContractState (v_Z := v_Z) (v_G := v_G) (n := n)) (t_Reject)) :=
   init_ovn_contract _  :=
-    Result_Ok (solve_lift (Build_t_OvnContractState (f_g_pow_xis := repeat (f_group_one (ret_both (tt : 'unit))) n) (f_zkp_xis := repeat (Build_t_SchnorrZKPCommit (f_schnorr_zkp_u := f_group_one (ret_both (tt : 'unit))) (f_schnorr_zkp_z := f_field_zero (ret_both (tt : 'unit))) (f_schnorr_zkp_c := f_field_zero (ret_both (tt : 'unit)))) n) (f_commit_vis := repeat (f_field_zero (ret_both (tt : 'unit))) n) (f_g_pow_xi_yi_vis := repeat (f_group_one (ret_both (tt : 'unit))) n) (f_zkp_vis := repeat (Build_t_OrZKPCommit (f_or_zkp_x := f_group_one (ret_both (tt : 'unit))) (f_or_zkp_y := f_group_one (ret_both (tt : 'unit))) (f_or_zkp_a1 := f_group_one (ret_both (tt : 'unit))) (f_or_zkp_b1 := f_group_one (ret_both (tt : 'unit))) (f_or_zkp_a2 := f_group_one (ret_both (tt : 'unit))) (f_or_zkp_b2 := f_group_one (ret_both (tt : 'unit))) (f_or_zkp_c := f_field_zero (ret_both (tt : 'unit))) (f_or_zkp_d1 := f_field_zero (ret_both (tt : 'unit))) (f_or_zkp_d2 := f_field_zero (ret_both (tt : 'unit))) (f_or_zkp_r1 := f_field_zero (ret_both (tt : 'unit))) (f_or_zkp_r2 := f_field_zero (ret_both (tt : 'unit)))) n) (f_tally := ret_both (0 : int32)))) : both (t_Result (t_OvnContractState (v_Z := v_Z) (v_G := v_G) (n := n)) (t_Reject)).
+    Result_Ok (solve_lift (Build_t_OvnContractState (f_g_pow_xis := repeat (f_group_one (ret_both (tt : 'unit))) n) (f_zkp_xis := repeat (Build_t_SchnorrZKPCommit (f_schnorr_zkp_u := f_group_one (ret_both (tt : 'unit))) (f_schnorr_zkp_z := f_field_zero (ret_both (tt : 'unit))) (f_schnorr_zkp_c := f_field_zero (ret_both (tt : 'unit)))) n) (f_commit_vis := repeat (f_field_zero (ret_both (tt : 'unit))) n) (f_g_pow_xi_yi_vis := repeat (f_group_one (ret_both (tt : 'unit))) n) (f_zkp_vis := repeat (Build_t_OrZKPCommit (f_or_zkp_x := f_group_one (ret_both (tt : 'unit))) (f_or_zkp_y := f_group_one (ret_both (tt : 'unit))) (f_or_zkp_a1 := f_group_one (ret_both (tt : 'unit))) (f_or_zkp_b1 := f_group_one (ret_both (tt : 'unit))) (f_or_zkp_a2 := f_group_one (ret_both (tt : 'unit))) (f_or_zkp_b2 := f_group_one (ret_both (tt : 'unit))) (f_or_zkp_c := f_field_zero (ret_both (tt : 'unit))) (f_or_zkp_d1 := f_field_zero (ret_both (tt : 'unit))) (f_or_zkp_d2 := f_field_zero (ret_both (tt : 'unit))) (f_or_zkp_r1 := f_field_zero (ret_both (tt : 'unit))) (f_or_zkp_r2 := f_field_zero (ret_both (tt : 'unit)))) n) (f_tally := ret_both (0 : int32)))) : both0 (t_Result (t_OvnContractState (v_Z := v_Z) (v_G := v_G) (n := n)) (t_Reject)).
 Fail Next Obligation.
 
-Equations register_vote {v_Z : _} {v_G : _} {n : both (uint_size)} {v_A : _} {impl_574521470_ : _} `{ t_Sized (v_Z)} `{ t_Sized (v_G)} `{ t_Sized (v_A)} `{ t_Sized (impl_574521470_)} `{ t_Z_Field (v_Z)} `{ t_Group (v_G) (v_Z)} `{ t_HasActions (v_A)} `{ t_HasReceiveContext (impl_574521470_) ('unit)} (ctx : both (impl_574521470_)) (state : both (t_OvnContractState (v_Z := v_Z) (v_G := v_G) (n := n))) : both (t_Result ((v_A × t_OvnContractState (v_Z := v_Z) (v_G := v_G) (n := n))) (t_ParseError)) :=
+Equations register_vote {v_Z : _} {v_G : _} {n : both0 (uint_size)} {v_A : _} {impl_574521470_ : _} `{ t_Sized (v_Z)} `{ t_Sized (v_G)} `{ t_Sized (v_A)} `{ t_Sized (impl_574521470_)} `{ t_Z_Field (v_Z)} `{ t_Group (v_G) (v_Z)} `{ t_HasActions (v_A)} `{ t_HasReceiveContext (impl_574521470_) ('unit)} (ctx : both0 (impl_574521470_)) (state : both0 (t_OvnContractState (v_Z := v_Z) (v_G := v_G) (n := n))) : both0 (t_Result ((v_A × t_OvnContractState (v_Z := v_Z) (v_G := v_G) (n := n))) (t_ParseError)) :=
   register_vote ctx state  :=
     solve_lift (run (letb '(_,out) := f_get (f_parameter_cursor ctx) in
     letm[choice_typeMonad.result_bind_code (t_Result ((v_A × t_OvnContractState (v_Z := v_Z) (v_G := v_G) (n := n))) (t_ParseError))] (params : t_RegisterParam (v_Z)) := matchb out with
@@ -454,12 +501,12 @@ Equations register_vote {v_Z : _} {v_G : _} {n : both (uint_size)} {v_A : _} {im
     letb register_vote_state_ret := f_clone state in
     letb register_vote_state_ret := Build_t_OvnContractState[register_vote_state_ret] (f_g_pow_xis := update_at_usize (f_g_pow_xis register_vote_state_ret) (cast_int (WS2 := _) (f_rp_i params)) g_pow_xi) in
     letb register_vote_state_ret := Build_t_OvnContractState[register_vote_state_ret] (f_zkp_xis := update_at_usize (f_zkp_xis register_vote_state_ret) (cast_int (WS2 := _) (f_rp_i params)) zkp_xi) in
-    Result_Ok (prod_b (f_accept (* (ret_both (tt : 'unit)) *),register_vote_state_ret))))) : both (t_Result ((v_A × t_OvnContractState (v_Z := v_Z) (v_G := v_G) (n := n))) (t_ParseError)).
+    Result_Ok (prod_b (f_accept (* (ret_both (tt : 'unit)) *),register_vote_state_ret))))) : both0 (t_Result ((v_A × t_OvnContractState (v_Z := v_Z) (v_G := v_G) (n := n))) (t_ParseError)).
 Fail Next Obligation.
 
-Equations tally_votes {v_Z : _} {v_G : _} {n : both (uint_size)} {v_A : _} {impl_574521470_ : _} `{ t_Sized (v_Z)} `{ t_Sized (v_G)} `{ t_Sized (v_A)} `{ t_Sized (impl_574521470_)} `{ t_Z_Field (v_Z)} `{ t_Group (v_G) (v_Z)} `{ t_HasActions (v_A)} `{ t_HasReceiveContext (impl_574521470_) ('unit)} (_ : both (impl_574521470_)) (state : both (t_OvnContractState (v_Z := v_Z) (v_G := v_G) (n := n))) : both (t_Result ((v_A × t_OvnContractState (v_Z := v_Z) (v_G := v_G) (n := n))) (t_ParseError)) :=
+Equations tally_votes {v_Z : _} {v_G : _} {n : both0 (uint_size)} {v_A : _} {impl_574521470_ : _} `{ t_Sized (v_Z)} `{ t_Sized (v_G)} `{ t_Sized (v_A)} `{ t_Sized (impl_574521470_)} `{ t_Z_Field (v_Z)} `{ t_Group (v_G) (v_Z)} `{ t_HasActions (v_A)} `{ t_HasReceiveContext (impl_574521470_) ('unit)} (_ : both0 (impl_574521470_)) (state : both0 (t_OvnContractState (v_Z := v_Z) (v_G := v_G) (n := n))) : both0 (t_Result ((v_A × t_OvnContractState (v_Z := v_Z) (v_G := v_G) (n := n))) (t_ParseError)) :=
   tally_votes _ state  :=
-    letb _ := foldi_both_list (f_into_iter (Build_t_Range (f_start := ret_both (0 : uint_size)) (f_end := n))) (fun i =>
+    letb _ := foldi_both0_list (f_into_iter (Build_t_Range (f_start := ret_both (0 : uint_size)) (f_end := n))) (fun i =>
       ssp (fun _ =>
         letb g_pow_yi := compute_g_pow_yi i (f_g_pow_xis state) in
         letm[choice_typeMonad.result_bind_code (t_Result ((v_A × t_OvnContractState (v_Z := v_Z) (v_G := v_G) (n := n))) (t_ParseError))] _ := ControlFlow_Continue (ifb negb (zkp_one_out_of_two_validate g_pow_yi ((f_zkp_vis state).a[i]))
@@ -469,24 +516,24 @@ Equations tally_votes {v_Z : _} {v_G : _} {n : both (uint_size)} {v_A : _} {impl
         solve_lift (ifb negb (check_commitment ((f_g_pow_xi_yi_vis state).a[i]) ((f_commit_vis state).a[i]))
         then letm[choice_typeMonad.result_bind_code (t_Result ((v_A × t_OvnContractState (v_Z := v_Z) (v_G := v_G) (n := n))) (t_ParseError))] hoist7 := v_Break (Result_Err (ret_both tt)) in
         ControlFlow_Continue (never_to_any hoist7)
-        else ControlFlow_Continue (ret_both (tt : 'unit))) : both _ (* (t_ControlFlow (t_Result ((v_A × t_OvnContractState (v_Z := v_Z) (v_G := v_G) (n := n))) (t_ParseError)) ('unit)) *))) (Ok (ret_both (tt : 'unit))) in
+        else ControlFlow_Continue (ret_both (tt : 'unit))) : both0 _ (* (t_ControlFlow (t_Result ((v_A × t_OvnContractState (v_Z := v_Z) (v_G := v_G) (n := n))) (t_ParseError)) ('unit)) *))) (Ok (ret_both (tt : 'unit))) in
     letb vote_result := f_group_one (ret_both (tt : 'unit)) in
-    letb vote_result := foldi_both_list ((* f_into_iter *) (array_to_list (f_g_pow_xi_yi_vis state))) (fun g_pow_vote =>
+    letb vote_result := foldi_both0_list ((* f_into_iter *) (array_to_list (f_g_pow_xi_yi_vis state))) (fun g_pow_vote =>
       ssp (fun vote_result =>
-        solve_lift (f_prod vote_result g_pow_vote) : both (f_group_type))) vote_result in
+        solve_lift (f_prod vote_result g_pow_vote) : both0 (f_group_type))) vote_result in
     letb tally := ret_both (0 : int32) in
     letb curr := f_field_zero (ret_both (tt : 'unit)) in
-    letb '(curr,tally) := foldi_both_list (f_into_iter (Build_t_Range (f_start := ret_both (0 : int32)) (f_end := cast_int (WS2 := _) n))) (fun i =>
+    letb '(curr,tally) := foldi_both0_list (f_into_iter (Build_t_Range (f_start := ret_both (0 : int32)) (f_end := cast_int (WS2 := _) n))) (fun i =>
       ssp (fun '(curr,tally) =>
         letb tally := ifb (f_g_pow curr) =.? vote_result
         then letb tally := i in
         tally
         else tally in
         letb curr := f_add curr (f_field_one (ret_both (tt : 'unit))) in
-        solve_lift (prod_b (curr,tally)) : both ((f_field_type × int32)))) (prod_b (curr,tally)) in
+        solve_lift (prod_b (curr,tally)) : both0 ((f_field_type × int32)))) (prod_b (curr,tally)) in
     letb tally_votes_state_ret := f_clone state in
     letb tally_votes_state_ret := Build_t_OvnContractState[tally_votes_state_ret] (f_tally := tally) in
-      Result_Ok (solve_lift (prod_b (f_accept (* (ret_both (tt : 'unit)) *),tally_votes_state_ret))) : both (t_Result ((v_A × t_OvnContractState (v_Z := v_Z) (v_G := v_G) (n := n))) (t_ParseError)).
+      Result_Ok (solve_lift (prod_b (f_accept (* (ret_both (tt : 'unit)) *),tally_votes_state_ret))) : both0 (t_Result ((v_A × t_OvnContractState (v_Z := v_Z) (v_G := v_G) (n := n))) (t_ParseError)).
 Solve All Obligations with now intros ; destruct from_uint_size.
 Fail Next Obligation.
 
@@ -506,40 +553,40 @@ Export Serializable.
 From Hacspec Require Import ConCertLib.
 Export ConCertLib.
 
-Definition state_OVN {v_Z : _} {v_G : _} {n : both (uint_size)} `{ t_Sized (v_Z)} `{ t_Sized (v_G)} `{ t_Z_Field (v_Z)} `{ t_Group (v_G) (v_Z)} : choice_type :=
+Definition state_OVN {v_Z : _} {v_G : _} {n : both0 (uint_size)} `{ t_Sized (v_Z)} `{ t_Sized (v_G)} `{ t_Z_Field (v_Z)} `{ t_Group (v_G) (v_Z)} : choice_type :=
   t_OvnContractState (v_Z := v_Z) (v_G := v_G) (n := n).
 
-#[global] Program Instance t_CastVoteParam_t_HasReceiveContext {v_Z : _} {v_G : _} {n : both (uint_size)} `{ t_Sized (v_Z)} `{ t_Sized (v_G)} `{ t_Z_Field (v_Z)} `{ t_Group (v_G) (v_Z)} : t_HasReceiveContext t_CastVoteParam 'unit :=
+#[global] Program Instance t_CastVoteParam_t_HasReceiveContext {v_Z : _} {v_G : _} {n : both0 (uint_size)} `{ t_Sized (v_Z)} `{ t_Sized (v_G)} `{ t_Z_Field (v_Z)} `{ t_Group (v_G) (v_Z)} : t_HasReceiveContext t_CastVoteParam 'unit :=
   {| f_get := (fun  {Ctx : _} => (solve_lift (@ret_both (t_ParamType × t_Result Ctx t_ParseError)) (tt, inr tt)) : _)|}.
 Fail Next Obligation.
-#[global] Program Instance t_CastVoteParam_t_Sized {v_Z : _} {v_G : _} {n : both (uint_size)} `{ t_Sized (v_Z)} `{ t_Sized (v_G)} `{ t_Z_Field (v_Z)} `{ t_Group (v_G) (v_Z)} : t_Sized t_CastVoteParam :=
+#[global] Program Instance t_CastVoteParam_t_Sized {v_Z : _} {v_G : _} {n : both0 (uint_size)} `{ t_Sized (v_Z)} `{ t_Sized (v_G)} `{ t_Z_Field (v_Z)} `{ t_Group (v_G) (v_Z)} : t_Sized t_CastVoteParam :=
   fun x =>
     x.
 Fail Next Obligation.
-Definition receive_OVN_cast_vote  {v_Z : _} {v_G : _} {n : both (uint_size)} `{ t_Sized (v_Z)} `{ t_Sized (v_G)} `{ t_Z_Field (v_Z)} `{ t_Group (v_G) (v_Z)} {v_A : _} `{ t_Sized (v_A)} `{ t_HasActions (v_A)} (ctx : both (t_CastVoteParam (v_Z := v_Z))) (st : both (state_OVN)) : both (t_Result ((v_A × state_OVN)) (t_ParseError)) :=
+Definition receive_OVN_cast_vote  {v_Z : _} {v_G : _} {n : both0 (uint_size)} `{ t_Sized (v_Z)} `{ t_Sized (v_G)} `{ t_Z_Field (v_Z)} `{ t_Group (v_G) (v_Z)} {v_A : _} `{ t_Sized (v_A)} `{ t_HasActions (v_A)} (ctx : both0 (t_CastVoteParam (v_Z := v_Z))) (st : both0 (state_OVN)) : both0 (t_Result ((v_A × state_OVN)) (t_ParseError)) :=
   cast_vote (v_Z := v_Z) (v_G := v_G) (n := n) (v_A := v_A)  (H2 := t_CastVoteParam_t_Sized (v_Z := v_Z) (v_G := v_G) (n := n))   (H7 := t_CastVoteParam_t_HasReceiveContext (v_Z := v_Z) (v_G := v_G) (n := n)) ctx st.
 
-(* #[global] Program Instance t_CastVoteParam_t_HasReceiveContext {v_Z : _} {v_G : _} {n : both (uint_size)} `{ t_Sized (v_Z)} `{ t_Sized (v_G)} `{ t_Z_Field (v_Z)} `{ t_Group (v_G) (v_Z)} : t_HasReceiveContext t_CastVoteParam 'unit := *)
+(* #[global] Program Instance t_CastVoteParam_t_HasReceiveContext {v_Z : _} {v_G : _} {n : both0 (uint_size)} `{ t_Sized (v_Z)} `{ t_Sized (v_G)} `{ t_Z_Field (v_Z)} `{ t_Group (v_G) (v_Z)} : t_HasReceiveContext t_CastVoteParam 'unit := *)
 (*   {| f_get := (fun  {Ctx : _} => (solve_lift (@ret_both (t_ParamType × t_Result Ctx t_ParseError)) (tt, inr tt)) : _)|}. *)
 (* Fail Next Obligation. *)
 (* #[global] Program Instance t_CastVoteParam_t_Sized : t_Sized t_CastVoteParam := *)
 (*   fun x => *)
 (*     x. *)
 (* Fail Next Obligation. *)
-Definition receive_OVN_commit_to_vote {v_Z : _} {v_G : _} {n : both (uint_size)} {v_A : _} (* {impl_574521470_ : _} *) `{ t_Sized (v_Z)} `{ t_Sized (v_G)} `{ t_Sized (v_A)} `{ t_Z_Field (v_Z)} `{ t_Group (v_G) (v_Z)} `{ t_HasActions (v_A)} (ctx : both (t_CastVoteParam)) (st : both (state_OVN (n := n))) : both (t_Result ((v_A × state_OVN)) (t_ParseError)) :=
+Definition receive_OVN_commit_to_vote {v_Z : _} {v_G : _} {n : both0 (uint_size)} {v_A : _} (* {impl_574521470_ : _} *) `{ t_Sized (v_Z)} `{ t_Sized (v_G)} `{ t_Sized (v_A)} `{ t_Z_Field (v_Z)} `{ t_Group (v_G) (v_Z)} `{ t_HasActions (v_A)} (ctx : both0 (t_CastVoteParam)) (st : both0 (state_OVN (n := n))) : both0 (t_Result ((v_A × state_OVN)) (t_ParseError)) :=
   commit_to_vote (H2 := t_CastVoteParam_t_Sized (n := n)) (H7 := t_CastVoteParam_t_HasReceiveContext (n := n)) ctx st.
 
-Definition init_OVN {v_Z : _} {v_G : _} {n : both (uint_size)} {v_A : _} (* {impl_574521470_ : _} *) `{ t_Sized (v_Z)} `{ t_Sized (v_G)} `{ t_Sized (v_A)} `{ t_Z_Field (v_Z)} `{ t_Group (v_G) (v_Z)} `{ t_HasActions (v_A)} (chain : Chain) (ctx : ContractCallContext) (st : state_OVN) : ResultMonad.result (state_OVN (n := n)) (t_ParseError) :=
+Definition init_OVN {v_Z : _} {v_G : _} {n : both0 (uint_size)} {v_A : _} (* {impl_574521470_ : _} *) `{ t_Sized (v_Z)} `{ t_Sized (v_G)} `{ t_Sized (v_A)} `{ t_Z_Field (v_Z)} `{ t_Group (v_G) (v_Z)} `{ t_HasActions (v_A)} (chain : Chain) (ctx : ContractCallContext) (st : state_OVN) : ResultMonad.result (state_OVN (n := n)) (t_ParseError) :=
   ResultMonad.Ok st.
 
-#[global] Program Instance t_RegisterParam_t_HasReceiveContext {v_Z : _} {v_G : _} {n : both (uint_size)} {v_A : _} (* {impl_574521470_ : _} *) `{ t_Sized (v_Z)} `{ t_Sized (v_G)} `{ t_Sized (v_A)} `{ t_Z_Field (v_Z)} `{ t_Group (v_G) (v_Z)} `{ t_HasActions (v_A)} : t_HasReceiveContext t_RegisterParam 'unit :=
+#[global] Program Instance t_RegisterParam_t_HasReceiveContext {v_Z : _} {v_G : _} {n : both0 (uint_size)} {v_A : _} (* {impl_574521470_ : _} *) `{ t_Sized (v_Z)} `{ t_Sized (v_G)} `{ t_Sized (v_A)} `{ t_Z_Field (v_Z)} `{ t_Group (v_G) (v_Z)} `{ t_HasActions (v_A)} : t_HasReceiveContext t_RegisterParam 'unit :=
   {| f_get := (fun  {Ctx : _} => (solve_lift (@ret_both (t_ParamType × t_Result Ctx t_ParseError)) (tt, inr tt)) : _)|}.
 Fail Next Obligation.
-#[global] Program Instance t_RegisterParam_t_Sized {v_Z : _} {v_G : _} {n : both (uint_size)} {v_A : _} (* {impl_574521470_ : _} *) `{ t_Sized (v_Z)} `{ t_Sized (v_G)} `{ t_Sized (v_A)} `{ t_Z_Field (v_Z)} `{ t_Group (v_G) (v_Z)} `{ t_HasActions (v_A)} : t_Sized t_RegisterParam :=
+#[global] Program Instance t_RegisterParam_t_Sized {v_Z : _} {v_G : _} {n : both0 (uint_size)} {v_A : _} (* {impl_574521470_ : _} *) `{ t_Sized (v_Z)} `{ t_Sized (v_G)} `{ t_Sized (v_A)} `{ t_Z_Field (v_Z)} `{ t_Group (v_G) (v_Z)} `{ t_HasActions (v_A)} : t_Sized t_RegisterParam :=
   fun x =>
     x.
 Fail Next Obligation.
-Definition receive_OVN_register {v_Z : _} {v_G : _} {n : both (uint_size)} {v_A : _} `{ t_Sized (v_Z)} `{ t_Sized (v_G)} `{ t_Sized (v_A)} `{ t_Z_Field (v_Z)} `{ t_Group (v_G) (v_Z)} `{ t_HasActions (v_A)}  (ctx : both (t_RegisterParam)) (st : both (state_OVN (n := n))) : both (t_Result ((v_A × state_OVN)) (t_ParseError)) :=
+Definition receive_OVN_register {v_Z : _} {v_G : _} {n : both0 (uint_size)} {v_A : _} `{ t_Sized (v_Z)} `{ t_Sized (v_G)} `{ t_Sized (v_A)} `{ t_Z_Field (v_Z)} `{ t_Group (v_G) (v_Z)} `{ t_HasActions (v_A)}  (ctx : both0 (t_RegisterParam)) (st : both0 (state_OVN (n := n))) : both0 (t_Result ((v_A × state_OVN)) (t_ParseError)) :=
   register_vote (H2 := t_RegisterParam_t_Sized (n := n)) (H7 := t_RegisterParam_t_HasReceiveContext (n := n)) ctx st.
 
 #[global] Program Instance t_TallyParameter_t_HasReceiveContext : t_HasReceiveContext t_TallyParameter 'unit :=
@@ -549,7 +596,7 @@ Fail Next Obligation.
   fun x =>
     x.
 Fail Next Obligation.
-Definition receive_OVN_tally {v_Z : _} {v_G : _} {n : both (uint_size)} {v_A : _} `{ t_Sized (v_Z)} `{ t_Sized (v_G)} `{ t_Sized (v_A)} `{ t_Z_Field (v_Z)} `{ t_Group (v_G) (v_Z)} `{ t_HasActions (v_A)} (ctx : both (t_TallyParameter)) (st : both (state_OVN)) : both (t_Result ((v_A × state_OVN (n := n))) (t_ParseError)) :=
+Definition receive_OVN_tally {v_Z : _} {v_G : _} {n : both0 (uint_size)} {v_A : _} `{ t_Sized (v_Z)} `{ t_Sized (v_G)} `{ t_Sized (v_A)} `{ t_Z_Field (v_Z)} `{ t_Group (v_G) (v_Z)} `{ t_HasActions (v_A)} (ctx : both0 (t_TallyParameter)) (st : both0 (state_OVN)) : both0 (t_Result ((v_A × state_OVN (n := n))) (t_ParseError)) :=
   tally_votes ctx st.
 
 Inductive Msg_OVN {v_Z : _} `{ t_Sized (v_Z)} `{ temp : t_Z_Field (v_Z)} : Type :=
@@ -557,39 +604,39 @@ Inductive Msg_OVN {v_Z : _} `{ t_Sized (v_Z)} `{ temp : t_Z_Field (v_Z)} : Type 
 | msg_OVN_commit_to_vote : t_CastVoteParam (v_Z := v_Z) (H0 := temp) -> Msg_OVN
 | msg_OVN_register : t_RegisterParam (v_Z := v_Z) -> Msg_OVN
 | msg_OVN_tally : t_TallyParameter -> Msg_OVN.
-#[global] Program Instance state_OVN_t_HasReceiveContext {v_Z : _} {v_G : _} {n : both (uint_size)} {v_A : _} (* {impl_574521470_ : _} *) `{ t_Sized (v_Z)} `{ t_Sized (v_G)} `{ t_Sized (v_A)} `{ t_Z_Field (v_Z)} `{ t_Group (v_G) (v_Z)} `{ t_HasActions (v_A)} : t_HasReceiveContext (state_OVN (n := n)) 'unit :=
+#[global] Program Instance state_OVN_t_HasReceiveContext {v_Z : _} {v_G : _} {n : both0 (uint_size)} {v_A : _} (* {impl_574521470_ : _} *) `{ t_Sized (v_Z)} `{ t_Sized (v_G)} `{ t_Sized (v_A)} `{ t_Z_Field (v_Z)} `{ t_Group (v_G) (v_Z)} `{ t_HasActions (v_A)} : t_HasReceiveContext (state_OVN (n := n)) 'unit :=
   {| f_get := (fun  (Ctx : _) => (solve_lift (@ret_both (t_ParamType × t_Result Ctx t_ParseError)) (tt, inr tt)) : _)|}.
 Fail Next Obligation.
-#[global] Program Instance state_OVN_t_Sized {v_Z : _} {v_G : _} {n : both (uint_size)} (* {impl_574521470_ : _} *) `{ t_Sized (v_Z)} `{ t_Sized (v_G)}  `{ t_Group (v_G) (v_Z)} : t_Sized (state_OVN (n := n)) :=
+#[global] Program Instance state_OVN_t_Sized {v_Z : _} {v_G : _} {n : both0 (uint_size)} (* {impl_574521470_ : _} *) `{ t_Sized (v_Z)} `{ t_Sized (v_G)}  `{ t_Group (v_G) (v_Z)} : t_Sized (state_OVN (n := n)) :=
   fun x =>
     x.
 Fail Next Obligation.
-#[global] Program Instance state_OVN_t_HasActions {v_Z : _} {v_G : _} {n : both (uint_size)}`{ t_Sized (v_Z)} `{ t_Sized (v_G)} `{ t_Group (v_G) (v_Z)} : t_HasActions (state_OVN (v_Z := v_Z) (n := n)).
+#[global] Program Instance state_OVN_t_HasActions {v_Z : _} {v_G : _} {n : both0 (uint_size)}`{ t_Sized (v_Z)} `{ t_Sized (v_G)} `{ t_Group (v_G) (v_Z)} : t_HasActions (state_OVN (v_Z := v_Z) (n := n)).
 Admit Obligations.
 Fail Next Obligation.
 Obligation Tactic := intros.
 
 (*  *)
-Equations receive_OVN  {v_Z : _} {v_G : _} {n : both (uint_size)} {v_A : _} `{ t_Sized (v_Z)} `{ t_Sized (v_G)} `{ t_Sized (v_A)} `{ temp1 : t_Z_Field (v_Z)} `{ t_Group (v_G) (v_Z)} `{ t_HasActions (v_A)} (chain : Chain) (ctx : ContractCallContext) (st : state_OVN (v_Z := v_Z) (n := n)) (msg : Datatypes.option (Msg_OVN  (v_Z := v_Z))) : ResultMonad.result (state_OVN (v_Z := v_Z) (n := n) * list ActionBody) t_ParseError :=
+Equations receive_OVN  {v_Z : _} {v_G : _} {n : both0 (uint_size)} {v_A : _} `{ t_Sized (v_Z)} `{ t_Sized (v_G)} `{ t_Sized (v_A)} `{ temp1 : t_Z_Field (v_Z)} `{ t_Group (v_G) (v_Z)} `{ t_HasActions (v_A)} (chain : Chain) (ctx : ContractCallContext) (st : state_OVN (v_Z := v_Z) (n := n)) (msg : Datatypes.option (Msg_OVN  (v_Z := v_Z))) : ResultMonad.result (state_OVN (v_Z := v_Z) (n := n) * list ActionBody) t_ParseError :=
   receive_OVN chain ctx st msg  :=
     match msg with
     | Some (msg_OVN_cast_vote val) =>
-      match is_pure (both_prog (@receive_OVN_cast_vote v_Z v_G n _ _ _ _ _ v_A _ _ (ret_both val) (ret_both st))) with
+      match is_pure (both0_prog (@receive_OVN_cast_vote v_Z v_G n _ _ _ _ _ v_A _ _ (ret_both val) (ret_both st))) with
          | inl x => ResultMonad.Ok ((snd x), [])
          | inr x => ResultMonad.Err x
          end
     | Some (msg_OVN_commit_to_vote val) =>
-    match is_pure (both_prog (@receive_OVN_commit_to_vote v_Z v_G n _ _ _ _ _ _ _ _ (ret_both val) (ret_both st))) with
+    match is_pure (both0_prog (@receive_OVN_commit_to_vote v_Z v_G n _ _ _ _ _ _ _ _ (ret_both val) (ret_both st))) with
          | inl x => ResultMonad.Ok ((snd x), [])
          | inr x => ResultMonad.Err x
          end
     | Some (msg_OVN_register val) =>
-      match is_pure (both_prog (@receive_OVN_register v_Z v_G n _ _ _ _ _ _ _ _ (ret_both val) (ret_both st))) with
+      match is_pure (both0_prog (@receive_OVN_register v_Z v_G n _ _ _ _ _ _ _ _ (ret_both val) (ret_both st))) with
          | inl x => ResultMonad.Ok ((snd x), [])
          | inr x => ResultMonad.Err x
          end
     | Some (msg_OVN_tally val) =>
-    match (is_pure (both_prog (@receive_OVN_tally v_Z v_G n _ _ _ _ _ _ _ _ (ret_both val) (ret_both st)))) with
+    match (is_pure (both0_prog (@receive_OVN_tally v_Z v_G n _ _ _ _ _ _ _ _ (ret_both val) (ret_both st)))) with
          | inl x => ResultMonad.Ok ((snd x), [])
          | inr x => ResultMonad.Err x
          end
@@ -597,7 +644,7 @@ Equations receive_OVN  {v_Z : _} {v_G : _} {n : both (uint_size)} {v_A : _} `{ t
       ResultMonad.Err tt
     end : ResultMonad.result (state_OVN (v_Z := v_Z) (n := n) * list ActionBody) t_ParseError.
 Fail Next Obligation.
-#[global] Program Instance state_OVN_Serializable  {v_Z : _} {v_G : _} {n : both (uint_size)} (* {impl_574521470_ : _} *) `{ t_Sized (v_Z)} `{ t_Sized (v_G)}  `{ t_Group (v_G) (v_Z)} : Serializable (state_OVN  (v_Z := v_Z) (n := n)) :=
+#[global] Program Instance state_OVN_Serializable  {v_Z : _} {v_G : _} {n : both0 (uint_size)} (* {impl_574521470_ : _} *) `{ t_Sized (v_Z)} `{ t_Sized (v_G)}  `{ t_Group (v_G) (v_Z)} : Serializable (state_OVN  (v_Z := v_Z) (n := n)) :=
   _.
 Admit Obligations.
 Fail Next Obligation.
@@ -605,4 +652,4 @@ Fail Next Obligation.
 Admit Obligations.
 (* Derive Serializable Msg_OVN_rect<msg_OVN_cast_vote,msg_OVN_commit_to_vote,msg_OVN_register,msg_OVN_tally>. *)
 Fail Next Obligation.
-Definition contract_OVN {v_Z : _} {v_G : _} {n : both (uint_size)} {v_A : _} `{ temp1 : t_Sized (v_Z)} `{ t_Sized (v_G)} `{ t_Sized (v_A)} `{ temp2 : t_Z_Field (v_Z)} `{ t_Group (v_G) (v_Z)} `{ t_HasActions (v_A)}  : @Contract _ (@state_OVN v_Z v_G n temp1 _ _ _ _) (@Msg_OVN v_Z temp1 H1 ) (state_OVN (v_Z := v_Z) (n := n)) (t_ParseError) state_OVN_Serializable Msg_OVN_Serializable state_OVN_Serializable _ := build_contract init_OVN receive_OVN.
+Definition contract_OVN {v_Z : _} {v_G : _} {n : both0 (uint_size)} {v_A : _} `{ temp1 : t_Sized (v_Z)} `{ t_Sized (v_G)} `{ t_Sized (v_A)} `{ temp2 : t_Z_Field (v_Z)} `{ t_Group (v_G) (v_Z)} `{ t_HasActions (v_A)}  : @Contract _ (@state_OVN v_Z v_G n temp1 _ _ _ _) (@Msg_OVN v_Z temp1 H1 ) (state_OVN (v_Z := v_Z) (n := n)) (t_ParseError) state_OVN_Serializable Msg_OVN_Serializable state_OVN_Serializable _ := build_contract init_OVN receive_OVN.
